finish verification for spinlock

Examples/SpinLock.v
@@ -231,8 +231,6 @@ Proof.
   }
 Qed.
 
-Module SpinLockTest.
-
 Definition E := CASSig bool.
 Definition F := LockSig.
 Definition acf T := @LockActiveMap T.
@@ -1443,7 +1441,7 @@ Proof.
   }
 Qed.
 
-Lemma SpinLock_all_return {T} : 
+Lemma SpinLock_all_return_aux {T} : 
   forall (i: Name T) A m v, ReturnStep i (Guar i) (Posts i A m v) m v (CSs i A m v).
 Proof.
   unfold ReturnStep.
@@ -1669,6 +1667,29 @@ Proof.
       }
     }
   }
+Qed.
+
+Lemma ReturnStepWeaken {T} i (A: Type) (m: F A) v P (G Q CS: (ReltU T)):
+  ReturnStep i G (ReltToPrec Q) m v CS -> 
+  ReturnStep i G (P <<- Q) m v CS.
+Proof.
+  intros.
+  unfold ReturnStep in *.
+  intros.
+  assert((ReltToPrec Q) s ρs).
+  { unfold PrecCompose in H0. destruct H0 as [s' [ρs' [? ?]]].
+    exists s', ρs'. easy.
+  }
+  specialize (H _ _ H2 H1).
+  assumption.
+Qed.
+
+Lemma SpinLock_all_return {T} : 
+  forall (i: Name T) A m v, ReturnStep i (Guar i) (Precs i A m <<-  Posts i A m v) m v (CSs i A m v).
+Proof.
+  intros. 
+  apply ReturnStepWeaken.
+  apply SpinLock_all_return_aux.
 Qed.
 
 Lemma SpinLock_verify_aux' {T} (i: Name T) A (m : LockSig A):
@@ -2700,592 +2721,485 @@ Proof.
   }
 Qed.
 
-Lemma SpinLock_Rel_aux1 {T} (i: Name T) (s1: InterState F (VE T)) ρs1 s2 ρs2: 
-  (prComp (Precs i unit Rel) (TInvoke SpinLockImpl i unit Rel)) s1 ρs1 s2 ρs2 ->
-    exists ρ, ρs2 = eq ρ /\ 
-    fst s2 i = Cont Rel (SpinLockImpl _ Rel) /\ 
-    PCalls ρ i = CallPoss Rel /\ PRets ρ i = RetIdle /\
-    ((snd s2 = CASDef (Some true) None /\ PState ρ = inl (LockOwned i))  \/ 
-     (PState ρ <> inl (LockOwned i) /\ (StateWithUB_acf _ (acf T) (PState ρ) i = None))).
-Proof.
-  intros.
-  destruct H.
-  unfold Precs in H.
-  destruct H as [ρ1 [? ?]].
-  unfold TInvoke in H0.
-  destruct_all.
-  exists (@MkPoss T F (VFU T) (PState ρ1)
-          (fun j => if i =? j then CallPoss Rel else PCalls ρ1 j)
-          (fun j => if i =? j then RetIdle else PRets ρ1 j)).
-  simpl.
-  split.
-  { subst ρs2. rewrite <- Poss_eq_inv2. rewrite H. reflexivity. }
-  split.
-  { unfold TIdle in H0. destruct_all. inversion H2; subst. 
-    simpl in H6. elim_corece. rewrite H0 in H6. 
-    inversion H6; subst. dependent destruction H4. easy. 
-  }
-  rewrite eqb_id.
-  do 2 split; try easy.
-  elim_corece.
-  rewrite H3 in H1.
-  destruct H1; [left | right]; easy.
-Qed.
-
-Lemma SpinLock_Rel_aux2 {T} (i: Name T) (s1: InterState F (VE T)) ρs1 s2 ρs2: 
-  (prComp (Precs i unit Rel) (TInvoke SpinLockImpl i unit Rel) ->> (Rely i)) s1 ρs1 s2 ρs2 ->
-    exists ρ, ρs2 = eq ρ /\ 
-    fst s2 i = Cont Rel (SpinLockImpl _ Rel) /\ 
-    PCalls ρ i = CallPoss Rel /\ PRets ρ i = RetIdle /\
-    ((snd s2 = CASDef (Some true) None /\ PState ρ = inl (LockOwned i))  \/ 
-     (PState ρ <> inl (LockOwned i) /\ (StateWithUB_acf _ (acf T) (PState ρ) i = None))).
-Proof.
-  intros.
-  destruct H as [s' [ρs' [? ?]]].
-  pose proof SpinLock_Rel_aux1 i s1 ρs1 s' ρs' H.
-  destruct H1 as [ρ' [? ?]].
-  unfold Rely in H0.
-  specialize (H0 _ H1).
-  destruct H0 as [ρ2 [? ?]].
-  exists ρ2.
-  split; try easy.
-  split.
-  { destruct_all. rewrite <- H3. rewrite H2. reflexivity. }
-  split.
-  { destruct_all. rewrite <- H10. apply H4. }
-  split.
-  { destruct_all. rewrite <- H11. apply H5. }
-  destruct_all.
-  destruct H6.
-  { destruct_all. specialize (H7 _ H13). destruct H7.
-    { left. destruct H7. rewrite <- H14, H7, H6. easy. }
-    { right. destruct H7 as [a ?]. rewrite <- H12. rewrite H7, H13. easy. }
-  }
-  { right. 
-    destruct H6. 
-    rewrite <- H12. rewrite H13.
-    split; [| reflexivity].
-    destruct (PState ρ').
-    { destruct s.
-      destruct owner.
-      { destruct (classicT (i = n)).
-        { subst n. specialize (H7 m (ltac:(auto))). destruct H7.
-          { destruct m.
-            { destruct H7. rewrite H7. easy. }
-            { unfold LockOwned in H6. contradiction. }
-          }
-          { destruct H7. rewrite H7. easy. }
-        }
-        { apply H8. intros. intro. inversion H14. subst n. contradiction. }
-      }
-      { apply H8. intros. intro. inversion H14. }
-    }
-    { destruct p. destruct u.
-      specialize (H9 a (ltac:(reflexivity))). destruct H9. rewrite H9. easy. 
-    }
-  }
-Qed.
-
-Lemma SpinLock_Rel_aux3 {T} (i: Name T) (s1: InterState F (VE T)) ρs1 s2 ρs2: 
-  ((prComp (Precs i unit Rel) (TInvoke SpinLockImpl i unit Rel) ->> (Rely i)) ->> 
-    (fun (s: InterState F (VE T)) (ρs: PossSet (VFU T)) t σs =>
-        exists ρ σ, ρs = eq ρ /\ σs = eq σ /\
-        UnderThreadStep (fst s i) (Some (CallEv (CAS (Some true) None))) (fst t i) /\
-        PCalls σ i = CallDone Rel /\
-        PRets σ i = RetIdle /\
-        ((PState ρ = inl (LockOwned i) /\ PState σ = inl (LockRelRan i) /\ Step (VE T) (snd s) (i, (CallEv (CAS (Some true) None))) (snd t)) \/ 
-         (exists a, PState σ = inr (UBState_, a) /\ (a i = Some (existT (fun A => LockSig A) unit Rel))))))
-    s1 ρs1 s2 ρs2 ->
-      exists ρ, ρs2 = eq ρ /\
-      fst s2 i = UCall Rel (CAS (Some true) None) (fun x1 : bool => Return x1;; Return tt) /\
-      PCalls ρ i = CallDone Rel /\
-      PRets ρ i = RetIdle /\
-      ((PState ρ = inl (LockRelRan i) /\ snd s2 = CASDef (Some true) (Some (MkCASPend i (CAS (Some true) None)))) \/
-       (exists a, PState ρ = inr (UBState_, a) /\ (a i = Some (existT (fun A => LockSig A) unit Rel)))).
-Proof.
-  intros.
-  destruct H as [s' [ρs' [? ?]]].
-  apply SpinLock_Rel_aux2 in H.
-  destruct H as [ρ [? [? [? [? ?]]]]].
-  destruct H0 as [ρ' [ρ2 [? [? ?]]]].
-  exists ρ2.
-  split; [easy |].
-  split.
-  { destruct H6. elim_corece. rewrite H1 in H6. inversion H6; subst.
-    dependent destruction H9. rewrite H13.
-    unfold call, ret in x.
-    rewrite ProgramFacts.frobProgId in x at 1. unfold ProgramFacts.frobProgram in x. simpl in x.
-    inversion x.
-    dependent destruction H5.
-    reflexivity.
-  }
-  split; [easy |].
-  split; [easy |].
-  destruct H6 as [? [? [? ?]]].
-  destruct H4.
-  { destruct H9.
-    { destruct H4. destruct H9. elim_corece. rewrite H4 in H11. destruct H11. inversion H12; subst. left. easy. }
-    { right. apply H9. } 
-  }
-  { pose proof Poss_eq_unique2 _ _ _ H H0. subst ρ.
-    destruct H9.
-    { destruct H9. destruct H4. contradiction. }
-    { right. destruct H9. exists x. easy. }
-  }
-Qed.
-
-Lemma SpinLock_Rel_aux4 {T} (i: Name T) (s1: InterState F (VE T)) ρs1 s2 ρs2 v: 
-  (((prComp (Precs i unit Rel) (TInvoke SpinLockImpl i unit Rel) ->> (Rely i)) ->> 
-    (fun (s: InterState F (VE T)) (ρs: PossSet (VFU T)) t σs =>
-        exists ρ σ, ρs = eq ρ /\ σs = eq σ /\
-        UnderThreadStep (fst s i) (Some (CallEv (CAS (Some true) None))) (fst t i) /\
-        PCalls σ i = CallDone Rel /\
-        PRets σ i = RetIdle /\
-        ((PState ρ = inl (LockOwned i) /\ PState σ = inl (LockRelRan i) /\ Step (VE T) (snd s) (i, (CallEv (CAS (Some true) None))) (snd t)) \/ 
-         (exists a, PState σ = inr (UBState_, a) /\ (a i = Some (existT (fun A => LockSig A) unit Rel)))))) ->>
-    (fun s ρs t σs =>
-        exists ρ σ, ρs = eq ρ /\ σs = eq σ /\
-        UnderThreadStep (fst s i) (Some (RetEv (CAS (Some true) None) v)) (fst t i) /\
-        PCalls σ i = CallDone Rel /\
-        PRets σ i = RetPoss Rel tt /\
-        ((PState ρ = inl (LockRelRan i) /\ (forall m, PState σ <> inl (LockDef (Some i) m))) \/ 
-         ((exists a, PState σ = inr (UBState_, a) /\ a i = None)))))
-    s1 ρs1 s2 ρs2 ->
-      exists ρ, ρs2 = eq ρ /\
-      fst s2 i = Cont Rel (Return tt) /\
-      PCalls ρ i = CallDone Rel /\
-      PRets ρ i = RetPoss Rel tt /\
-      ((forall m, PState ρ <> inl (LockDef (Some i) m)) \/ 
-      (exists a, PState ρ = inr (UBState_, a) /\ a i = None)).
-Proof.
-  intros.
-  destruct H as [s' [ρs' [? ?]]].
-  apply SpinLock_Rel_aux3 in H.
-  destruct H as [ρ [? [? [? [? ?]]]]].
-  destruct H0 as [ρ' [ρ2 [? [? ?]]]].
-  exists ρ2.
-  split; [easy |].
-  split.
-  { destruct H6. elim_corece. rewrite H1 in H6. inversion H6; subst.
-    dependent destruction H9. dependent destruction H12. rewrite H14.
-    rewrite (ProgramFacts.frobProgId (@Return (CASSig bool) bool v;; Return tt)).
-    unfold ProgramFacts.frobProgram.
-    simpl. reflexivity.    
-  }
-  split; [easy |].
-  split; [easy |].
-  destruct H6 as [? [? [? ?]]].
-  destruct H4.
-  { destruct H9.
-    { destruct H9. left. apply H10. }
-    { destruct H9. right. exists x. easy. }
-  }
-  { pose proof Poss_eq_unique2 _ _ _ H H0. subst ρ.
-    destruct H9.
-    { destruct H9. left. easy. }
-    { right. destruct H9. exists x. easy. }
-  }
-Qed.
-
-Lemma SpinLock_Rel_verified {T} : 
+Lemma SpinLock_Rel_verified {T} :
   forall (i: Name T), 
       VerifyProg i (Rely i) (Guar i) 
       (prComp (Precs i unit Rel) (TInvoke SpinLockImpl i _ Rel) ->> Rely i)
       (SpinLockImpl _ Rel)
       (Posts i unit Rel).
 Proof.
-  intros. simpl.
-  apply (lemBind (fun (_: bool) => 
-            (fun v : unit => Posts i unit Rel v) tt)).
-  + eapply weakenPost.
-    eapply (lemCall 
-      (Q := fun (s: InterState F (VE T)) (ρs: PossSet (VFU T)) t σs =>
-        exists ρ σ, ρs = eq ρ /\ σs = eq σ /\
-        UnderThreadStep (fst s i) (Some (CallEv (CAS (Some true) None))) (fst t i) /\
-        PCalls σ i = CallDone Rel /\
-        PRets σ i = RetIdle /\
-        ((PState ρ = inl (LockOwned i) /\ PState σ = inl (LockRelRan i) /\ Step (VE T) (snd s) (i, (CallEv (CAS (Some true) None))) (snd t)) \/ 
-         (exists a, PState σ = inr (UBState_, a) /\ (a i = Some (existT (fun A => LockSig A) unit Rel)))))
-      (S := fun v s ρs t σs =>
-        exists ρ σ, ρs = eq ρ /\ σs = eq σ /\
-        UnderThreadStep (fst s i) (Some (RetEv (CAS (Some true) None) v)) (fst t i) /\
-        PCalls σ i = CallDone Rel /\
-        PRets σ i = RetPoss Rel tt /\
-        (((PState ρ = inl (LockRelRan i) /\ forall m, PState σ <> inl (LockDef (Some i) m))) \/ 
-         (exists a, PState σ = inr (UBState_, a) /\ a i = None)))).
-    { unfold Stable, stableRelt, sub, subRelt.
-      intros.
-      rename ρ into ρs.
-      rename σ into σs.
-      destruct H as [s' [ρs' [? ?]]].
-      destruct H as [ρ [ρ' [? [? ?]]]].
-      unfold Rely in H0.
-      specialize (H0 _ H1).
-      destruct H0 as [σ [? ?]].
-      exists ρ, σ.
-      split; try easy.
-      split; try easy.
-      split.
-      { destruct H2. destruct H3. elim_corece. rewrite <- H3. apply H2. }
-      split.
-      { destruct_all. unfold F. rewrite <- H7. easy. }
-      split.
-      { destruct_all. unfold F. rewrite <- H8. easy. }  
-      destruct_all.
-      destruct H12.
-      { destruct H12 as [? [? ?]].
-        specialize (H4 _ H13).
-        destruct H4.
-        { left. destruct H4. elim_corece. rewrite <- H15. easy. }
-        { right. destruct H4 as [a ?].
-          unfold F in H13.
-          rewrite H13 in H9.
-          rewrite H4 in H9.
-          inversion H9; subst. rewrite eqb_id in H16.
-          exists a. easy.
-        }
-      }
-      {
-        right.
-        destruct H12 as [a ?].
-        destruct H12.
-        specialize (H6 _ H12).
-        destruct H6 as [a' ?].
-        unfold F in H12.
-        rewrite H12 in H9.
-        exists a'.
-        split; try easy.
-        rewrite H6 in H9.
-        inversion H9; subst.
-        easy.
-      }
+  intros.
+  simpl.
+  unfold SpinLockRel.
+  rewrite SpinLock_verify_aux.
+  apply weakenPrec with (P := 
+    fun _ _ s ρs => exists (ρ: Poss (VFU T)), ρs = eq ρ /\
+      StateWithUB_acf _ (acf T) (PState ρ) i = None /\
+      (((PCalls ρ i = CallPoss Rel /\ PRets ρ i = RetIdle) /\
+        (fst s i = Cont Rel (SpinLockImpl unit Rel)) /\
+        (i_owns i s ρ \/ i_not_owns i s ρ \/ unowns_acq i s ρ \/ i_owns_rel i s ρ)) \/ 
+      (((PCalls ρ i = CallPoss Rel /\ PRets ρ i = RetIdle) /\
+          is_ub_state s ρ)))).
+  2: {
+    unfold sub, subRelt.
+    intros.
+    rename ρ into ρs.
+    rename σ into σs.
+    destruct H as [ρ [σ [? [? ?]]]].
+    exists σ.
+    repeat split; try easy.
+    destruct_all.
+    destruct H9 as [Howns | [Hunowns | [Hunowns_acq | [Howns_rel | Hub]]]].
+    { destruct Howns as [Howns HT].
+      destruct HT.
+      { left. split; [easy |]. split; [easy |]. left. easy. }
+      { right. split; [| easy]. easy. }
     }
-    { unfold Stable, stablePost, stableRelt, sub, subRelt.
-      intros.
-      rename ρ into ρs.
-      rename σ into σs.
-      destruct H as [s' [ρs' [? ?]]].
-      destruct H as [ρ [ρ' [? [? ?]]]].
-      unfold Rely in H0.
-      specialize (H0 _ H1).
-      destruct H0 as [σ [? ?]].
-      exists ρ, σ.
-      split; try easy.
-      split; try easy.
-      split.
-      { destruct H2. destruct H3. elim_corece. rewrite <- H3. apply H2. }
-      split.
-      { destruct_all. unfold F. rewrite <- H7. easy. }
-      split.
-      { destruct_all. unfold F. rewrite <- H8. easy. }  
-      destruct_all.
-      destruct H12.
-      { destruct H12 as [? ?].
-        specialize (H5 H13).
-        left. easy. 
-      }
-      { right.
-        destruct H12 as [a [? ?]].
-        specialize (H6 _ H12).
-        destruct H6 as [a' ?].
-        exists a'.
-        unfold F in H12.
-        rewrite H12 in H9.
-        rewrite H6 in H9.
-        inversion H9; subst.
-        easy.
-      }
+    { destruct Hunowns as [Hunowns HT].
+      destruct HT.
+      { left. split; [easy |]. split; [easy |]. right. left. easy. }
+      { right. split; [| easy]. easy. }
     }
-    { unfold Commit. intros.
-      destruct H as [s0 [ρs0 ?]].
-      apply SpinLock_Rel_aux2 in H.
-      destruct H as [ρ [? [? [? [? ?]]]]].
-      destruct H6.
-      {
-        remember (
-          (MkPoss T LockSig (VFU T)
-          (inl (LockRelRan i))
-          (fun k : Name T =>
-            match @eqb (Name T) i k
-            return (PCall LockSig) with
-            | true => @CallDone LockSig unit Rel
-            | false => @PCalls T LockSig (VFU T) ρ k
-            end)
-          (fun k : Name T =>
-            match @eqb (Name T) i k
-            return (PRet LockSig) with
-            | true => @RetIdle LockSig
-            | false => @PRets T LockSig (VFU T) ρ k
-            end))) as σ.
-        exists (eq σ).
-        split. { exists σ. easy. }
-        split.
-        { intros. subst σ0. exists ρ.
-          split. { rewrite H. reflexivity. }
-          subst σ.
-          destruct ρ.
-          destruct_all. simpl in *. subst.
-          eapply PossStepsStep.
-          4: apply PossStepsRefl.
-          { apply PCommitCall with (i := i) (A := unit) (m := Rel); simpl; try easy.
-            { constructor. constructor. }
-            { rewrite eqb_id. easy. }
-            { rewrite eqb_id. easy. }
-          }
-          { intros. simpl. rewrite (eqb_nid _ _ H). easy. }
-          { intros. simpl. rewrite (eqb_nid _ _ H). easy. }
-        }
-        split.
-        { exists ρ, σ.
-          subst σ. simpl. rewrite eqb_id. 
-          repeat split; try easy.
-          left. easy.
-        }
-        {
-          unfold Guar.
+    { destruct Hunowns_acq as [Hunowns_acq HT].
+      destruct HT.
+      { left. split; [easy |]. split; [easy |]. right. right. left. easy. }
+      { right. split; [| easy]. easy. }
+    }
+    { destruct Howns_rel as [Howns_rel HT].
+      destruct HT.
+      { left. split; [easy |]. split; [easy |]. right. right. right. easy. }
+      { right. split; [| easy]. easy. }
+    }
+    { right. split; [| easy]. easy. }
+  }
+  eapply lemBind.
+  { eapply (lemCall
+      (Q := fun s ρs t σs => exists (ρ σ: Poss (VFU T)), ρs = eq ρ /\ σs = eq σ /\
+              StateWithUB_acf _ (acf T) (PState ρ) i = None /\
+              StateWithUB_acf _ (acf T) (PState σ) i = None /\
+              ((PCalls ρ i = CallPoss Rel /\ PRets ρ i = RetIdle /\
+                PCalls σ i = CallPoss Rel /\ PRets σ i = RetIdle /\
+                fst s i = Cont Rel (SpinLockImpl unit Rel) /\
+                fst t i = UCall Rel (CAS (Some true) None) (fun x : bool => Return x;; ret tt) /\
+                ((i_owns i s ρ /\ i_owns_rel i t σ))) \/
+              (((PCalls σ i = CallPoss Rel /\ PRets σ i = RetIdle) \/
+                (PCalls σ i = CallDone Rel /\ PRets σ i = RetPoss Rel tt)) /\
+                is_ub_state t σ)))
+      (S := fun v s ρs t σs => exists (ρ σ: Poss (VFU T)), ρs = eq ρ /\ σs = eq σ /\
+              StateWithUB_acf _ (acf T) (PState ρ) i = None /\
+              StateWithUB_acf _ (acf T) (PState σ) i = None /\                  
+              (((fst s i = UCall Rel (CAS (Some true) None) (fun x : bool => Return x;; ret tt)) /\
+                ((v = true /\ PCalls ρ i = CallPoss Rel /\ PRets ρ i = RetIdle /\
+                    PCalls σ i = CallDone Rel /\ PRets σ i = RetPoss Rel tt /\
+                    fst t i = Cont Rel (Return tt) /\
+                    ((i_owns_rel i s ρ /\ i_not_owns i t σ))))) \/
+                (((PCalls σ i = CallPoss Rel /\ PRets σ i = RetIdle) \/
+                  (PCalls σ i = CallDone Rel /\ PRets σ i = RetPoss Rel tt)) /\
+                  is_ub_state t σ)))).
+        { unfold Stable, stableRelt, sub, subRelt.
           intros.
-          pose proof Poss_eq_unique2 _ _ _ H H7. subst ρ0.
-          exists σ.
-          split; try easy.
-          split.
-          { unfold differ_pointwise in H0. intros. specialize (H0 j (ltac:(auto))). easy. }
-          split.
-          { intros.
-            rewrite H9 in H6.
-            destruct H6.
-            inversion H10; subst; contradiction. 
+          rename ρ into ρs.
+          rename σ into σs.
+          destruct H as [s' [ρs' [? ?]]].
+          destruct H as [ρ [ρ' [Hρ [Hρ' ?]]]].
+          destruct H as [Hstateρ [Hstateρ' Hpos]].
+          unfold Rely in H0.
+          specialize (H0 _ Hρ').
+          destruct H0 as [σ [Hσ H0]].
+          destruct H0 as [Hfstt [Howns [Hnotowns [Howns_rel [Howns_acq [Hother_owns_acq Hub]]]]]].
+          destruct Hub as [Hub [HPcallρ' [HPretρ' Hstateσ]]].
+          exists ρ, σ.
+          elim_corece. rewrite <- Hstateσ.
+          repeat split; try easy.
+          destruct Hpos as [HH | HH].
+          { destruct HH as [HPcallρi [HRetsρi [HCallsρ [HRetsρ [Hfsts [Hfsts' HH]]]]]].
+            elim_corece. rewrite <- Hfstt, <- HPcallρ', <- HPretρ'. 
+            { destruct HH as [Howns' Howns_rel'].
+              specialize (Howns_rel Howns_rel'). destruct Howns_rel as [Howns_rel | Hub']. 
+              { left. do 6 (split; [easy |]). easy. } 
+              { right. split; [| easy]. left. easy. }
+            }
           }
-          split.
-          { intros. subst σ. simpl. intro. inversion H10; subst; contradiction. }
-          split.
-          { intros. rewrite H8 in H6. destruct H6. inversion H9. }
-          { intros. subst σ. simpl. assert(i <> j) by easy.
-            rewrite (eqb_nid _ _ H9). destruct H6. rewrite H10. easy.
-          }
+          { right. destruct HH as [? HH]. specialize (Hub HH). split;[| easy]. 
+            rewrite <- HPcallρ', <- HPretρ'. easy. }
         }
-      }
-      { 
-        remember
-          ((MkPoss T LockSig (VFU T)
-          (inr (UBState_, fun j => if i =? j then Some (existT (fun A => LockSig A) unit Rel) else (StateWithUB_acf _ (acf T) (PState ρ) j)))
-          (fun j => if i =? j then CallDone Rel else PCalls ρ j)
-          (fun j => if i =? j then RetIdle else PRets ρ j))) as σ.
-        exists (eq σ).
-        split. { exists σ. easy. }
-        split.
-        { intros. subst σ0. exists ρ.
-          split. { rewrite H. reflexivity. }
-          subst σ.
-          destruct ρ.
-          destruct_all. simpl in *. subst.
-          eapply PossStepsStep.
-          4: apply PossStepsRefl.
-          { apply PCommitCall with (i := i) (A := unit) (m := Rel); simpl; try easy.
-            { destruct PState.
-              { constructor.
-                { intros. intro. inversion H; subst. contradiction. }
-                { constructor; try rewrite eqb_id; try easy; try apply differ_pointwise_trivial. }
+        { unfold Stable, stablePost, stableRelt, sub, subRelt. 
+          intros.
+          rename ρ into ρs.
+          rename σ into σs.
+          destruct H as [s' [ρs' [? ?]]].
+          destruct H as [ρ [ρ' [Hρ [Hρ' ?]]]].
+          destruct H as [Hstateρ [Hstateρ' Hpos]].
+          unfold Rely in H0.
+          specialize (H0 _ Hρ').
+          destruct H0 as [σ [Hσ H0]].
+          destruct H0 as [Hfstt [Howns [Hnotowns [Howns_rel [Howns_acq [Hother_owns_acq Hub]]]]]].
+          destruct Hub as [Hub [HPcallρ' [HPretρ' Hstateσ]]].
+          exists ρ, σ.
+          elim_corece. rewrite <- Hstateσ, <- HPcallρ', <- HPretρ', <- Hfstt.
+          do 4 (split; [easy |]).
+          destruct Hpos as [HH | HH].
+          { destruct HH as [Hfsts HH].
+            destruct HH as [Hv [HCallρ [HRetρ [HCallsρ' [HRetsρ' [Hfsts' HH]]]]]].
+            destruct HH as [Hsρ HH].
+            specialize (Hnotowns HH). destruct Hnotowns. 
+              { left. split; [easy |]. easy. }
+              { right. split; [| easy]. right. easy. }
+          }
+          { right. destruct HH as [? HH]. specialize (Hub HH). split; easy. }
+        }
+        { unfold Commit. intros.
+          destruct H as [s0 [ρs0 [ρ [Hρ [Hstateρ HPrec]]]]].
+          destruct HPrec as [HPrec | HH].
+          { destruct HPrec as [[HPcallρ HPRetsρ] [Hfsts HPrec]].
+            assert(fst t i = UCall Rel (CAS (Some true) None) (fun x : bool => Return x;; ret tt)) as Hfstt.
+            { elim_corece. rewrite Hfsts in H1. inversion H1. subst.
+              dependent destruction H3. rewrite frobProgId in x at 1. cbn in x. dependent destruction x. easy.
+            }
+            assert(
+              (PState ρ = inl (LockOwned i) /\ snd s = CASDef (Some true) None) \/
+              (PState ρ = inl (LockUnowned) /\ snd s = CASDef None None) \/
+              (exists j, j <> i /\ PState ρ = inl (LockOwned j) /\ snd s = CASDef (Some true) None)) as HCases.
+            {
+              destruct HPrec as [Howns | [Hunowns | [Hunowns_acq | Howns_rel]]].
+              { left. unfold i_owns in Howns. destruct Howns as [Howns Hsnds].
+                destruct Hsnds.
+                { easy. }
+                { destruct H as [j [Hneq Hsnds]].
+                  elim_corece. rewrite Hsnds in H2. inversion H2.
+                }
               }
-              { destruct p as [u a]. destruct u.
-                simpl in H7.
-                constructor.
-                constructor; try rewrite eqb_id; try easy; try apply differ_pointwise_trivial.
+              { unfold i_not_owns in Hunowns.
+                destruct Hunowns as [Hother_owns | [Hunowns | [Hunowns_acq | Hother_owns_rel]]].
+                { unfold other_owns in Hother_owns. destruct Hother_owns as [j [Hneq Hother_owns]].
+                  destruct Hother_owns as [Howns Hsnds].
+                  destruct Hsnds.
+                  { right. right. exists j. easy. }
+                  { destruct H as [j0 [Hneq' Hsnds]].
+                    elim_corece. rewrite Hsnds in H2. inversion H2.
+                  }
+                }
+                { right. left. unfold i_not_owns in Hunowns. destruct Hunowns as [Hunowns Hsnds].
+                  destruct Hsnds. easy.
+                }
+                { unfold unowns_acq in Hunowns_acq. 
+                  destruct Hunowns_acq as [j [Hneq [Hstate Hsnds]]].
+                  elim_corece. rewrite Hsnds in H2. inversion H2.
+                }
+                { unfold other_owns_rel in Hother_owns_rel. 
+                  destruct Hother_owns_rel as [j [Hneq [Hstate Hsnds]]].
+                  elim_corece. rewrite Hsnds in H2. inversion H2.
+                }
+              }
+              { unfold unowns_acq in Hunowns_acq. 
+                destruct Hunowns_acq as [Hstate Hsnds].
+                elim_corece. rewrite Hsnds in H2. inversion H2.
+              }
+              { unfold i_owns_rel in Howns_rel. destruct Howns_rel as [Howns_rel Hsnds].
+                elim_corece. rewrite Hsnds in H2. inversion H2.
               }
             }
-            { rewrite eqb_id. easy. }
-            { rewrite eqb_id. easy. }
+            destruct HCases as [HH | [HH | HH]].
+            { exists ρs.
+              destruct HH as [Hstate Hsnds].
+              rewrite Hsnds in H2. inversion H2; subst.
+              split. { exists ρ. easy. }
+              split.
+              { intros σ Hσ. subst σ.
+                exists ρ. split. { reflexivity. }
+                constructor.
+              } 
+              split.
+              { 
+                exists ρ, ρ.
+                repeat split; try easy.
+                left. do 5 (split; [easy |]). split; [easy |].
+                split.
+                { unfold i_owns. split; [easy |]. left. easy. }
+                { unfold i_owns_rel. easy. }
+              }
+              { unfold Guar.
+                assert(i_owns i s ρ) as Howns. { unfold i_owns. split; [easy |]. left. easy. }
+                intros ρ' Hρ'.
+                pose proof Poss_eq_unique3 _ _ Hρ'; subst ρ'. clear Hρ'.
+                exists ρ.
+                repeat split; try easy; intros.
+                { unfold differ_pointwise in H0. specialize (H0 j (ltac:(easy))). easy. }
+                { destruct Howns as [Hi ?]. destruct H3 as [Hj ?].
+                  rewrite Hi in Hj. inversion Hj. subst j. congruence.
+                }
+                { left. unfold i_not_owns. right. right. right.
+                  exists i. split; [easy |].
+                  unfold i_owns_rel. easy.
+                }
+                { assert (i_not_owns j s ρ) as Hnotowns. { left. exists i. easy. }
+                  pose proof inotowns_iownsrel_exclusive _ _ _ Hnotowns H3. contradiction.
+                }
+                { destruct H3. elim_corece. rewrite H4 in Hsnds. inversion Hsnds. }
+                { destruct H3 as [j0 [Hneq' [? H4]]]. elim_corece. rewrite H4 in Hsnds. inversion Hsnds. }
+                { apply is_ub_state_easy with (s := s) (ρ := ρ); easy. }
+              }
+            }
+            { destruct HH as [Hstate Hsnds].
+              assert(is_ub_state t (stateStepToUB ρ i Rel tt)) as Hub.
+              { unfold is_ub_state. simpl. 
+                exists (StateWithUB_acf LockStep (acf T) (PState ρ)).
+                split; [easy |].
+                eexists. eexists. elim_corece. 
+                rewrite Hsnds in H2. inversion H2; subst.
+                elim_corece. rewrite <- H7. reflexivity.
+              }
+              exists (eq (stateStepToUB ρ i Rel tt)).
+              split.
+              { eexists. reflexivity. }
+              split.
+              { intros. subst σ. exists ρ.
+                split. { rewrite Hρ. reflexivity. }
+                apply stateStepToUBPossSteps; try easy.
+                rewrite Hstate. constructor.
+                { intros. intro. inversion H. }
+                { econstructor; try rewrite eqb_id; try easy.
+                  unfold differ_pointwise. intros j Hneq. rewrite eqb_nid. 2: easy.
+                  rewrite Hstate. easy.
+                }
+              }
+              split.
+              { exists ρ, (stateStepToUB ρ i Rel tt).
+                repeat split; try easy.
+                right. try easy. split; [| easy].
+                right. unfold stateStepToUB. simpl. rewrite eqb_id. easy.
+              }
+              { unfold Guar. intros ρ' Hρ'.
+                pose proof Poss_eq_unique2 _ _ _ Hρ Hρ'; subst ρ'. clear Hρ'.
+                eexists. split; [reflexivity |].
+                split. { apply differ_pointwise_other. easy. } 
+                split. { intros. right. easy. } 
+                split. { intros. right. easy. }
+                split. { intros. right. easy. }
+                split. { intros. right. easy. }
+                split. { intros. right. easy. } 
+                split. { intros. easy. }
+                split. { intros. unfold stateStepToUB. simpl. rewrite eqb_nid; easy. }
+                { intros. unfold stateStepToUB. simpl. easy. }
+              }
+            }
+            { destruct HH as [j [Hneq [Hstate Hsnds]]].
+              assert(is_ub_state t (stateStepToUB ρ i Rel tt)) as Hub.
+              { unfold is_ub_state. simpl. 
+                exists (StateWithUB_acf LockStep (acf T) (PState ρ)).
+                split; [easy |].
+                eexists. eexists. elim_corece. 
+                rewrite Hsnds in H2. inversion H2; subst.
+                elim_corece. rewrite <- H7. reflexivity.
+              }
+              exists (eq (stateStepToUB ρ i Rel tt)).
+              split.
+              { eexists. reflexivity. }
+              split.
+              { intros. subst σ. exists ρ.
+                split. { rewrite Hρ. reflexivity. }
+                apply stateStepToUBPossSteps; try easy.
+                rewrite Hstate. constructor.
+                { intros. intro. inversion H; subst. congruence. }
+                { econstructor; try rewrite eqb_id; try easy.
+                  unfold differ_pointwise. intros j' Hneq'. rewrite eqb_nid. 2: easy.
+                  rewrite Hstate. easy.
+                }
+              }
+              split.
+              { exists ρ, (stateStepToUB ρ i Rel tt).
+                repeat split; try easy.
+                right. try easy. split; [| easy].
+                right. unfold stateStepToUB. simpl. rewrite eqb_id. easy.
+              }
+              { unfold Guar. intros ρ' Hρ'.
+                pose proof Poss_eq_unique2 _ _ _ Hρ Hρ'; subst ρ'. clear Hρ'.
+                eexists. split; [reflexivity |].
+                split. { apply differ_pointwise_other. easy. } 
+                split. { intros. right. easy. } 
+                split. { intros. right. easy. }
+                split. { intros. right. easy. }
+                split. { intros. right. easy. }
+                split. { intros. right. easy. } 
+                split. { intros. easy. }
+                split. { intros. unfold stateStepToUB. simpl. rewrite eqb_nid; easy. }
+                { intros. unfold stateStepToUB. simpl. easy. }
+              }
+            }
           }
-          { intros. simpl. rewrite (eqb_nid _ _ H). easy. }
-          { intros. simpl. rewrite (eqb_nid _ _ H). easy. }
+          { pose proof HH as Hub. unfold is_ub_state in HH.
+            destruct HH as [a [Hstate [o [mm Hsnds]]]].
+            assert(is_ub_state t ρ) as Hub'.
+            { apply is_ub_state_easy with (s := s)(ρ := ρ); easy. }
+            exists (eq ρ).
+            split.
+            { eexists. reflexivity. }
+            split.
+            { intros. subst σ. exists ρ.
+              split. { rewrite Hρ. reflexivity. }
+              constructor.
+            }
+            split.
+            { exists ρ, ρ.
+              repeat split; try easy.
+              right. split; [| easy]. 
+              left. easy.
+            }
+            { unfold Guar. intros ρ' Hρ'.
+              pose proof Poss_eq_unique2 _ _ _ Hρ Hρ'; subst ρ'. clear Hρ'.
+              eexists. split; [reflexivity |].
+              split. { apply differ_pointwise_other. easy. } 
+              split. { intros. right. easy. } 
+              split. { intros. right. easy. }
+              split. { intros. right. easy. }
+              split. { intros. right. easy. }
+              split. { intros. right. easy. }
+              split. { intros. easy. }
+              split. { intros. easy. }
+              { intros. easy. }
+            }
+          }
         }
-        split.
-        { exists ρ, σ.
-          subst σ. simpl. rewrite eqb_id. 
-          repeat split; try easy.
-          right.
-          eexists.
-          split.
-          { reflexivity. }
-          { simpl. rewrite eqb_id. easy. }
+        { intros v.
+          unfold Commit. intros.
+          destruct H as [s0 [ρs0 [s1 [ρs1 ?]]]].
+          destruct H as [HPrec HPost].
+          destruct HPrec as [ρ1 [Hρ1 [Hstateρ1 HPrec]]].
+          destruct HPost as [ρ1' [ρ [Hρ1' [Hρ [Hstateρ1' [Hstateρ HPost]]]]]].
+          assert((PCalls ρ i = CallPoss Rel /\ PRets ρ i = RetIdle /\  
+                 (fst s i = UCall Rel (CAS (Some true) None) (fun x : bool => Return x;; ret tt)) /\
+                  (i_owns i s1 ρ1' /\ i_owns_rel i s ρ)) \/
+                 (((PCalls ρ i = CallPoss Rel /\ PRets ρ i = RetIdle) \/
+                   (PCalls ρ i = CallDone Rel /\ PRets ρ i = RetPoss Rel tt)) /\
+                  is_ub_state s ρ)) as HPost'.
+          { destruct HPost as [HH | HH].
+            { destruct HH as [HCallsρ1' [HRetsρ1' [HCallsρ [HRetsρ [Hfsts1 [Hfsts HH]]]]]].
+              { left. split; [easy |]. split; [easy |]. split; [easy |]. easy. }
+            }
+            { right. easy. }
+          }
+          clear HPost.
+          destruct HPost' as [HCommit | Hub].
+          { destruct HCommit as [PCallsρ [PRetsρ [Hfsts HSucc]]].
+            { destruct HSucc as [_ HSucc].
+              pose proof HSucc as HSucc'.
+              unfold i_owns_rel in HSucc.
+              destruct HSucc as [HSρ HSs].
+              elim_corece. rewrite HSs in H2.
+              unfold CAS_i_rel in H2.
+              inversion H2; subst. 2: contradiction.
+              dependent destruction H7.
+              rewrite Hfsts in H1. inversion H1; subst.
+              dependent destruction H3. dependent destruction H6.
+              rewrite frobProgId in H9 at 1. cbn in H9.
+              remember (@MkPoss T F (VFU T) (inl (LockRelRan i)) 
+                      (fun j => if i =? j then CallDone Rel else PCalls ρ j)
+                      (fun j => if i =? j then RetIdle else PRets ρ j)) as ρ'.
+              remember (@MkPoss T F (VFU T) (inl (LockUnowned)) 
+                      (fun j => if i =? j then CallDone Rel else PCalls ρ' j)
+                      (fun j => if i =? j then RetPoss Rel tt else PRets ρ' j)) as ρ''.
+              exists (eq ρ'').
+              split. { eexists. reflexivity. }
+              split.
+              { intros. subst σ. exists ρ.
+                split. { reflexivity. }
+                eapply Logic.PossStepsStep with (i := i) (σ := ρ').
+                { subst ρ'. 
+                  apply Logic.PCommitCall with (m := Rel); simpl; try rewrite eqb_id; try easy.
+                  { rewrite HSρ. constructor. constructor. }
+                }
+                { subst ρ'. intros. simpl. rewrite eqb_nid; easy. }
+                { subst ρ'. intros. simpl. rewrite eqb_nid; easy. }
+                eapply Logic.PossStepsStep with (i := i) (σ := ρ'').
+                { subst ρ''. subst ρ'.
+                  apply Logic.PCommitRet with (m := Rel)(v := tt); simpl; try rewrite eqb_id; try easy.
+                  { simpl. constructor. constructor. }
+                }
+                { subst ρ''. intros. simpl. rewrite eqb_nid; easy. }
+                { subst ρ''. intros. simpl. rewrite eqb_nid; easy. }
+                constructor.
+              }
+              split.
+              { exists ρ, ρ''.
+                repeat split; try easy.
+                { subst ρ''. simpl. easy. }
+                { left. subst ρ''. simpl. rewrite eqb_id. repeat split; try easy. right. left. easy. } 
+              }
+              { unfold Guar. intros ρ_ Hρ_.
+                pose proof Poss_eq_unique3 _ _ Hρ_; subst ρ_. clear Hρ_.
+                eexists. split; [reflexivity |].
+                split. { apply differ_pointwise_other. easy. } 
+                split. { intros. destruct H3 as [HH ?]. rewrite HSρ in HH. inversion HH. subst j. congruence. }
+                split. 
+                { intros. left. right. left.
+                  subst ρ''. split; [easy |]. easy.
+                }
+                split. { intros. destruct H3 as [HH ?]. rewrite HSρ in HH. inversion HH. subst j; congruence. }
+                split. { intros. destruct H3 as [? HH]. elim_corece. rewrite HSs in HH. inversion HH. }
+                split. { intros. destruct H3 as [? [j0 [? HH]]]. elim_corece. rewrite HSs in HH. inversion HH. }
+                split. { intros. destruct H as [a [HH ?]]. elim_corece. rewrite HSρ in HH. inversion HH. }
+                split. { intros. subst ρ''. subst ρ'. simpl. rewrite eqb_nid; easy. }
+                { intros. subst ρ''. subst ρ'. simpl. rewrite HSρ. easy. }
+              }
+            }
+          }
+          { destruct Hub as [? Hub]. pose proof Hub as Hub'.
+            destruct Hub as [a [HUρ [m [o HPus]]]].
+            rewrite HUρ in Hstateρ. inversion Hstateρ. simpl in *.
+            assert(is_ub_state t ρ) as HUbt.
+            { apply is_ub_state_easy with (s := s)(ρ := ρ); easy. }
+            exists (eq ρ).
+            split. { eexists. reflexivity. }
+            split. { intros. subst σ. exists ρ. split; [subst ρs; easy | ]. constructor. }
+            split.
+            { exists ρ, ρ. 
+              repeat split; try rewrite HUρ; try easy.
+              right. repeat split; try easy.
+            }
+            { unfold Guar. intros ρ' Hρ'.
+              pose proof Poss_eq_unique2 _ _ _ Hρ Hρ'; subst ρ'. clear Hρ'.
+              eexists. split; [reflexivity |].
+              split. { apply differ_pointwise_other. easy. } 
+              split. { intros. right. easy. }
+              split. { intros. right. easy. }
+              split. { intros. right. easy. }
+              split. { intros. right. easy. }
+              split. { intros. right. easy. }
+              split. { intros. easy. }
+              split. { intros. easy. }
+              { intros. easy. }
+            }
+          }
         }
-        {
-          unfold Guar.
-          intros.
-          pose proof Poss_eq_unique2 _ _ _ H H7. subst ρ0.
-          exists σ.
-          split; try easy.
-          split.
-          { unfold differ_pointwise in H0. intros. specialize (H0 j (ltac:(auto))). easy. }
-          split.
-          { intros. right. subst σ. eexists. reflexivity. }
-          split.
-          { intros. subst σ. simpl. easy. }
-          split.
-          { intros. subst σ. eexists. reflexivity. }
-          { intros. subst σ. simpl. assert(i <> j) by easy.
-            rewrite (eqb_nid _ _ H9). destruct H6. easy. }
-        }
-      }
+  }
+  { intros. apply lemRet.
+    unfold sub, subRelt.
+    intros.
+    rename σ into σs.
+    rename ρ into ρs.
+    destruct H as [s2 [ρs2 [H0 H]]].
+    destruct H as [s1 [ρs1 [H1 H]]].
+    clear H0 H1.
+    destruct H as [ρ1 [σ [Hρ1 [Hσ H]]]].
+    destruct H as [Hstateρ1 [Hstateσ H]].
+    unfold Posts.
+    exists σ.
+    split; [easy |].
+    destruct H as [HH | HH].
+    { left.
+      destruct HH as [Hfsts1 [Hv [HCallsρ1 [HRetsρ1 [HCallsσ [HRetsσ [Hfstt Howns_rel]]]]]]].
+      subst v. repeat split; easy.
     }
-    {
-      unfold Commit. intros.
-      destruct H as [s0 [ρs0 ?]].
-      apply SpinLock_Rel_aux3 in H.
-      destruct H as [ρ [? [? [? [? ?]]]]].
-      destruct H6.
-      {
-        remember (
-          (MkPoss T LockSig (VFU T)
-          (inl (LockUnowned))
-          (fun k : Name T =>
-            match @eqb (Name T) i k
-            return (PCall LockSig) with
-            | true => @CallDone LockSig unit Rel
-            | false => @PCalls T LockSig (VFU T) ρ k
-            end)
-          (fun k : Name T =>
-            match @eqb (Name T) i k
-            return (PRet LockSig) with
-            | true => @RetPoss LockSig unit Rel tt
-            | false => @PRets T LockSig (VFU T) ρ k
-            end))) as σ.
-        exists (eq σ).
-        split. { exists σ. easy. }
-        split.
-        { intros. subst σ0. exists ρ.
-          split. { rewrite H. reflexivity. }
-          subst σ.
-          destruct ρ.
-          destruct_all. simpl in *. subst.
-          eapply PossStepsStep.
-          4: apply PossStepsRefl.
-          { apply PCommitRet with (i := i) (A := unit) (m := Rel) (v := tt); simpl; try easy.
-            { constructor. constructor. }
-            { rewrite eqb_id. easy. }
-            { rewrite eqb_id. easy. }
-          }
-          { intros. simpl. rewrite (eqb_nid _ _ H). easy. }
-          { intros. simpl. rewrite (eqb_nid _ _ H). easy. }
-        }
-        split.
-        { exists ρ, σ.
-          subst σ. simpl. rewrite eqb_id. 
-          repeat split; try easy.
-          left. easy.
-        }
-        {
-          unfold Guar.
-          intros.
-          pose proof Poss_eq_unique2 _ _ _ H H7. subst ρ0.
-          exists σ.
-          split; try easy.
-          split.
-          { unfold differ_pointwise in H0. intros. specialize (H0 j (ltac:(auto))). easy. }
-          split.
-          { intros.
-            rewrite H9 in H6.
-            destruct H6.
-            inversion H6; subst; contradiction. 
-          }
-          split.
-          { intros. subst σ. simpl. intro. inversion H10; subst; contradiction. }
-          split.
-          { intros. rewrite H8 in H6. destruct H6. inversion H6. }
-          { intros. subst σ. simpl. assert(i <> j) by easy.
-            destruct H6. rewrite H6. simpl.
-            rewrite (eqb_nid _ _ H9). 
-            easy.
-          }
-        }
-      }
-      {
-        remember
-          ((MkPoss T LockSig (VFU T)
-          (inr (UBState_, fun j => if i =? j then None else (StateWithUB_acf _ (acf T) (PState ρ) j)))
-          (fun j => if i =? j then CallDone Rel else PCalls ρ j)
-          (fun j => if i =? j then RetPoss Rel tt else PRets ρ j))) as σ.
-        exists (eq σ).
-        split. { exists σ. easy. }
-        split.
-        { intros. subst σ0. exists ρ.
-          split. { rewrite H. reflexivity. }
-          subst σ.
-          destruct ρ.
-          destruct_all. simpl in *. subst.
-          eapply PossStepsStep.
-          4: apply PossStepsRefl.
-          { apply PCommitRet with (i := i) (A := unit) (m := Rel) (v := tt); simpl; try easy.
-            { constructor. constructor; try rewrite eqb_id; try easy; try apply differ_pointwise_trivial. }
-            { rewrite eqb_id. easy. }
-            { rewrite eqb_id. easy. }
-          }
-          { intros. simpl. rewrite (eqb_nid _ _ H). easy. }
-          { intros. simpl. rewrite (eqb_nid _ _ H). easy. }
-        }
-        split.
-        { exists ρ, σ.
-          subst σ. simpl. rewrite eqb_id. 
-          repeat split; try easy.
-          right.
-          eexists.
-          split.
-          { reflexivity. }
-          { simpl. rewrite eqb_id. easy. }
-        }
-        {
-          unfold Guar.
-          intros.
-          pose proof Poss_eq_unique2 _ _ _ H H7. subst ρ0.
-          exists σ.
-          split; try easy.
-          split.
-          { unfold differ_pointwise in H0. intros. specialize (H0 j (ltac:(auto))). easy. }
-          split.
-          { intros. right. subst σ. eexists. reflexivity. }
-          split.
-          { intros. subst σ. simpl. easy. }
-          split.
-          { intros. subst σ. eexists. reflexivity. }
-          { intros. subst σ. simpl. assert(i <> j) by easy.
-            rewrite (eqb_nid _ _ H9). destruct H6. easy. }
-        }
-      }
+    { right.
+      destruct HH as [HH Hub].
+      split; [| easy].
+      easy.
     }
-    {
-      unfold sub, subRelt.
-      intros.
-      rewrite <- LogicFacts.reltCompAssoc in H.
-      rename ρ into ρs.
-      rename σ into σs.
-      assert(Precs i unit Rel s ρs).
-      { destruct H as [x1 [x2 [? ?]]].
-        destruct H as [x3 [x4 [? ?]]].
-        destruct H as [x5 [x6 [? ?]]].
-        unfold prComp in H.
-        destruct H.
-        apply H.
-      }
-      apply SpinLock_Rel_aux4 in H.
-      unfold Posts.
-      unfold Precs in H0.
-      destruct H0 as [ρ [? ?]].
-      destruct H as [σ [? ?]].
-      exists ρ, σ.
-      split; try easy.
-      split; try easy.
-      split; try easy.
-      destruct H2 as [? [? [? ?]]].
-      destruct H5.
-      { left. easy. }
-      { right. destruct H5 as [a [? ?]]. exists a. easy. }
-    }
-  + intros.
-    constructor.
-    easy.
+  }
 Qed.
 
-Lemma SpinLock_all_verified {T} : 
-  forall (i: Name T) A m, 
+Lemma SpinLock_all_verified {T A} :
+  forall (i: Name T) (m: F A), 
       VerifyProg i (Rely i) (Guar i) 
       (prComp (Precs i A m) (TInvoke SpinLockImpl i _ m) ->> Rely i)
       (SpinLockImpl _ m)
@@ -3293,1561 +3207,31 @@ Lemma SpinLock_all_verified {T} :
 Proof.
   intros.
   destruct m.
-  + apply SpinLock_Acq_verified.
-  + apply SpinLock_Rel_verified.
+  { apply SpinLock_Acq_verified. }
+  { apply SpinLock_Rel_verified. }
 Qed.
 
-Lemma SpinLock_all_return {T} : 
-  forall (i: Name T) A m v, ReturnStep i (Guar i) (Posts i A m v) m v (CSs i A m v).
+Definition SpinLockLayer {T} := ((VE T) :> SpinLockImpl).
+
+Theorem SpinLockCorrect {T} :
+  VerifyImpl (SpinLockLayer.(USpec)) (VFU T) Rely Guar Precs (LImpl (T := T) SpinLockLayer) Posts CSs.
 Proof.
-  intros.
-  destruct m.
-  + admit.
-  + unfold ReturnStep.
-    intros.
-    unfold Posts in H.
-    destruct H as [s1 [ρs1 [ρ1 [ρ ?]]]].
-    destruct_all.
-    exists ρs.
-    split.
-    { exists ρ. rewrite H1. easy. }
-    split.
-    { intros. exists σ. split; [exact H5 | constructor]. }
-    split.
-    { intros. pose proof Poss_eq_unique _ _ _ H1 H5. subst σ. destruct v. easy. }
-    split.
-    { unfold CSs. 
-      exists ρ.
-      exists (MkPoss T F (VFU T)
-        (PState ρ)
-        (fun j => if i =? j then CallIdle else PCalls ρ j)
-        (fun j => if i =? j then RetIdle else PRets ρ j)).
-      split; [easy |].
-      split.
-      { extensionality x. apply propositional_extensionality. split; intros.
-        { destruct H5 as [σ [? ?]]. pose proof Poss_eq_unique _ _ _ H1 H5. subst σ. destruct v.
-          unfold mapRetPoss in H6.
-          destruct x. destruct ρ.
-          simpl in *.
-          destruct_all.
-          f_equal.
-          { easy. }
-          { extensionality j. destruct (classicT (i = j)).
-            { subst j. rewrite eqb_id. rewrite H6. easy. }
-            { rewrite (eqb_nid _ _ n). unfold differ_pointwise in H10.
-              assert(j <> i) by auto.
-              specialize (H10 j H13). easy.
-            }
-          }
-          { extensionality j. destruct (classicT (i = j)).
-            { subst j. rewrite eqb_id. rewrite H8. easy. }
-            { rewrite (eqb_nid _ _ n). unfold differ_pointwise in H11.
-              assert(j <> i) by auto.
-              specialize (H11 j H13). easy.
-            }
-          }
-        }
-        { exists ρ.
-          split. { rewrite H1. reflexivity. } 
-          unfold mapRetPoss.
-          subst x. simpl. rewrite eqb_id.
-          destruct v.
-          repeat split; try apply differ_pointwise_trivial; easy.
-        }
-      }
-      simpl. rewrite eqb_id.
-      repeat split; try apply differ_pointwise_trivial; easy.
-    }
-    { unfold Guar. intros.
-      pose proof Poss_eq_unique2 _ _ _ H1 H5. subst ρ0.
-      exists (MkPoss T F (VFU T)
-        (PState ρ)
-        (fun j => if i =? j then CallIdle else PCalls ρ j)
-        (fun j => if i =? j then RetIdle else PRets ρ j)).
-      split.
-      { extensionality x. apply propositional_extensionality. split; intros.
-        { destruct H6 as [σ [? ?]]. pose proof Poss_eq_unique _ _ _ H1 H6. subst σ. destruct v.
-          unfold mapRetPoss in H7.
-          destruct x. destruct ρ.
-          simpl in *.
-          destruct_all.
-          f_equal.
-          { easy. }
-          { extensionality j. destruct (classicT (i = j)).
-            { subst j. rewrite eqb_id. rewrite H7. easy. }
-            { rewrite (eqb_nid _ _ n). unfold differ_pointwise in H11.
-              assert(j <> i) by auto.
-              specialize (H11 j H14). easy.
-            }
-          }
-          { extensionality j. destruct (classicT (i = j)).
-            { subst j. rewrite eqb_id. rewrite H9. easy. }
-            { rewrite (eqb_nid _ _ n). unfold differ_pointwise in H12.
-              assert(j <> i) by auto.
-              specialize (H12 j H14). easy.
-            }
-          }
-        }
-        { exists ρ.
-          split. { rewrite H1. reflexivity. } 
-          unfold mapRetPoss.
-          subst x. simpl. rewrite eqb_id.
-          destruct v.
-          repeat split; try apply differ_pointwise_trivial; easy.
-        }
-      }
-      simpl.
-      split.
-      { intros. assert(i <> j) by auto. rewrite (eqb_nid _ _ H7). easy. }
-      split.
-      { intros. left. easy. }
-      split.
-      { intros. apply H7. }
-      split.
-      { intros. exists a1. easy. }
-      split.
-      { assert(i <> j) by auto. rewrite (eqb_nid _ _ H7). easy. }
-      split.
-      { assert(i <> j) by auto. rewrite (eqb_nid _ _ H7). easy. }
-      { reflexivity. }
-    }
-Admitted.
-
-End SpinLockTest.
-
-Module SpinLockNormal.
-
-Definition E := CASSig bool.
-Definition F := LockSig.
-Definition VE T : Spec T E:= @casSpec T bool.
-Definition VF T := @lockSpec T.
-Definition Relt T := Relt (VE T) (VF T).
-Definition Prec T := Prec (VE T) (VF T).
-Definition Post T := Post (VE T) (VF T).
-
-(* Definition Valid {T} : Prec T :=
-  fun s ρs => exists ρ, ρs = eq ρ /\
-    ((PState ρ = LockUnowned /\ exists m, snd s = CASDef None m) \/
-    (exists j, PState ρ = LockAcqRan j /\ exists m, snd s = CASDef None m) \/
-    (exists j, PState ρ = LockOwned j /\ exists m, snd s = CASDef (Some true) m) \/
-    (exists j, PState ρ = LockRelRan j /\ exists m, snd s = CASDef (Some true) m)).
-
-Definition Invalid {T} : Prec T :=
-  fun s ρs => ~Valid s ρs. *)
-
-Definition Precs {T} i A (m : LockSig A) : Prec T :=
-  fun s ρs => exists ρ, ρs = eq ρ /\
-    match m with
-    | Acq =>
-        (PState ρ <> LockOwned i /\ PState ρ <> LockRelRan i /\ PState ρ <> LockAcqRan i)
-    | Rel =>
-        PState ρ = LockOwned i /\ snd s = CASDef (Some true) None
-    end.
-
-Definition Posts {T} i A (m : LockSig A) : Post T A :=
-  fun v s ρs t σs => exists ρ σ, ρs = eq ρ /\ σs = eq σ /\
-    match m with
-    | Acq =>
-        (PState σ = LockOwned i /\ PState ρ <> LockOwned i)
-    | Rel =>
-        PState ρ = LockOwned i /\
-        (forall m, PState σ <> LockDef (Some i) m) /\
-        σ.(PRets) i = RetPoss m v /\
-        σ.(PCalls) i = CallDone m /\
-        fst t i = Cont m (Return v)
-    end.
-
-Definition Rely {T} i : Relt T :=
-  fun s ρs t σs => forall ρ, ρs = eq ρ -> exists σ, σs = eq σ /\
-    (PCalls ρ i = PCalls σ i) /\
-    (PRets ρ i = PRets σ i) /\
-    (forall m, PState ρ = LockDef (Some i) m -> PState σ = LockDef (Some i) m) /\ 
-    (forall m, PState ρ = LockDef (Some i) m -> snd s = snd t) /\
-    ((forall m, PState ρ <> LockDef (Some i) m) -> (forall m, PState σ <> LockDef (Some i) m)) /\
-    (fst s i = fst t i).
-
-Definition Guar {T} i : Relt T :=
-  fun s ρs t σs => forall ρ, ρs = eq ρ -> exists σ, σs = eq σ /\
-    (forall j, j <> i -> fst s j = fst t j) /\
-    (forall j, j <> i -> PCalls ρ j = PCalls σ j) /\
-    (forall j, j <> i -> PRets ρ j = PRets σ j) /\
-    (forall j, j <> i -> 
-      forall m, PState ρ = LockDef (Some j) m -> PState σ = LockDef (Some j) m) /\
-    (forall j, j <> i -> 
-      forall m, PState ρ = LockDef (Some j) m -> snd s = snd t) /\
-    (forall j, j <> i -> 
-      ((forall m, PState ρ <> LockDef (Some j) m) -> (forall m, PState σ <> LockDef (Some j) m))).
-
-Lemma SpinLock_R_refl {T} : forall (i : Name T) s ρ, Rely i s ρ s ρ.
-Proof.
-  unfold Rely; intros.
-  exists ρ0.
-  split; auto.
-  repeat split; intros; auto.
+  constructor.
+  { apply SpinLock_R_refl. }
+  { apply SpinLock_R_trans. }
+  { apply SpinLock_G_in_R. }
+  { apply SpinLock_Inv_in_R. }
+  { apply SpinLock_Ret_in_R. }
+  { apply SpinLock_init_in_P. }
+  { apply SpinLock_P_stable. }
+  { apply SpinLock_switch_code. }
+  { simpl. intros. apply SpinLock_all_verified. }
+  { intros. apply SpinLock_all_return. }
 Qed.
 
-Lemma SpinLock_R_trans {T} : 
-  forall (i : Name T), Rely i ->> Rely i ==> Rely i.
+Theorem SpinLock_Linearizable {T} :
+  Lin (overObj SpinLockLayer) (VFU T).
 Proof.
-  unfold sub, subRelt.
-  intros.
-  unfold ReltCompose in H.
-  destruct_all.
-  rename x into s'.
-  rename x0 into ρ'.
-  unfold Rely in *.
-  intros.
-  specialize (H ρ0 H1).
-  destruct_all.
-  rename x into ρ'_.
-  specialize (H0 ρ'_ H).
-  destruct_all.
-  rename x into σ_.
-  exists σ_.
-  repeat split; intros; try easy.
-Admitted.
-
-Lemma SpinLock_G_in_R {T} : 
-  forall (i j : Name T), i <> j -> Guar i ==> Rely j.
-Proof.
-  unfold Guar, Rely, sub, subRelt. intros.
-  specialize (H0 _ H1).
-  destruct_all.
-  exists x.
-  specialize (H2 j (ltac: (easy))).
-  specialize (H3 j (ltac: (easy))).
-  specialize (H4 j (ltac: (easy))).
-  specialize (H5 j (ltac: (easy))).
-  specialize (H6 j (ltac: (easy))).
-  specialize (H7 j (ltac: (easy))).
-  repeat split; intros; try easy.
-  + specialize (H5 m).
-    apply H5, H8.
-  + specialize (H5 m).
-    apply (H6 _ H8).
-  + apply H7, H8.
+  eapply soundness.
+  apply SpinLockCorrect.
 Qed.
-
-Lemma Poss_eq_inv: forall {T A VF} (i: Name T) (m : LockSig A) ρs ρ σs (σ: Poss VF),
-  ρs = eq ρ ->
-  σs = (fun σ  =>
-        exists ρ,
-        ρs ρ /\
-        PState σ = PState ρ /\
-        PCalls σ i = CallPoss m /\
-        PRets σ i = RetIdle /\
-        differ_pointwise (PCalls ρ) (PCalls σ) i /\
-        differ_pointwise (PRets ρ) (PRets σ) i) ->
-  σ = {| PState := PState ρ; PCalls :=
-        fun k : Name T =>
-          if i =? k then CallPoss m 
-          else PCalls ρ k; PRets :=
-        fun k : Name T =>
-          if i =? k then RetIdle 
-          else PRets ρ k |} ->
-  σs = eq σ.
-Proof.
-  intros.
-  rewrite H0, H1.
-  extensionality σ'.
-  apply propositional_extensionality.
-  split.
-  { 
-    clear H0 H1.
-    intros.
-    destruct H0 as [ρ' [? [? [? [? [? ?]]]]]].
-    assert(ρ = ρ'). { rewrite H in H0. apply H0. }
-    subst ρ'.
-    destruct σ'; simpl in *.
-    apply f_equal3.
-    { auto. }
-    { 
-      extensionality k. destruct (classicT (i = k)).
-      { subst k. rewrite eqb_id. auto. }
-      { 
-        rewrite (eqb_nid _ _ n).
-        unfold differ_pointwise in H4.
-        specialize (H4 k (ltac:(auto))).
-        auto.
-      }
-    }
-    { 
-      extensionality k. destruct (classicT (i = k)).
-      { subst k. rewrite eqb_id. auto. }
-      { 
-        rewrite (eqb_nid _ _ n).
-        unfold differ_pointwise in H5.
-        specialize (H5 k (ltac:(auto))).
-        auto.
-      }
-    }
-  }
-  {
-    intros. subst σ'.
-    exists ρ.
-    repeat split.
-    { rewrite H. reflexivity. }
-    { simpl. rewrite eqb_id. reflexivity. } 
-    { simpl. rewrite eqb_id. reflexivity. }
-    { simpl. apply differ_pointwise_trivial. }
-    { simpl. apply differ_pointwise_trivial. }
-  }
-Qed.
-
-Lemma Poss_eq_inv2: forall {T A VF} (i: Name T) (m : LockSig A) ρs ρ (σs: PossSet VF),
-  ρs = eq ρ ->
-  σs = (fun σ =>
-        exists ρ,
-        ρs ρ /\
-        PState σ = PState ρ /\
-        PCalls σ i = CallPoss m /\
-        PRets σ i = RetIdle /\
-        differ_pointwise (PCalls ρ) (PCalls σ) i /\
-        differ_pointwise (PRets ρ) (PRets σ) i) ->
-  σs = eq {| PState := PState ρ; PCalls :=
-        fun k : Name T =>
-          if i =? k then CallPoss m 
-          else PCalls ρ k; PRets :=
-        fun k : Name T =>
-          if i =? k then RetIdle 
-          else PRets ρ k |}.
-Proof.
-  intros.
-  pose proof Poss_eq_inv i m ρs ρ σs 
-    {| PState := PState ρ; 
-       PCalls := fun j : Name T => if i =? j then CallPoss m else PCalls ρ j; 
-       PRets := fun j : Name T => if i =? j then RetIdle else PRets ρ j |} H H0.
-    apply H1.
-    reflexivity.
-Qed.
-
-Lemma Poss_eq_inv3: forall {F T} {VF: Spec T F} (i: Name T) (ρ: Poss VF) σs (st: State VF) pcall pret,
-  σs = (fun σ =>
-        PState σ = st /\
-        PCalls σ i = pcall /\
-        PRets σ i = pret /\
-        differ_pointwise (PCalls ρ) (PCalls σ) i /\
-        differ_pointwise (PRets ρ) (PRets σ) i) ->
-  σs = eq ( {| PState := st; 
-        PCalls := fun k : Name T => if i =? k then pcall else PCalls ρ k; 
-        PRets :=  fun k : Name T => if i =? k then pret else PRets ρ k |} : Poss VF).
-Proof.
-  intros.
-  extensionality σ'.
-  apply propositional_extensionality.
-  split.
-  { 
-    intros.
-    rewrite H in H0.
-    destruct H0 as [? [? [? [? ?]]]].
-    destruct σ'; simpl in *.
-    unfold differ_pointwise in H3, H4.
-    f_equal; try easy.
-    { extensionality k.
-      destruct (classicT (i = k)).
-      { subst k. rewrite eqb_id. auto. }
-      { rewrite (eqb_nid _ _ n). specialize (H3 k (ltac:(auto))). auto. }
-    }
-    { extensionality k.
-      destruct (classicT (i = k)).
-      { subst k. rewrite eqb_id. auto. }
-      { rewrite (eqb_nid _ _ n). specialize (H4 k (ltac:(auto))). auto. }
-    }
-  }
-  {
-    intros.
-    subst σ'.
-    rewrite H.
-    simpl.
-    rewrite eqb_id.
-    repeat split; auto.
-    { apply differ_pointwise_trivial. }
-    { apply differ_pointwise_trivial. }
-  }
-Qed.
-
-Lemma Poss_eq_unique: forall {T} ρs (ρ: Poss (VF T)) ρ', 
-  ρs = eq ρ -> ρs ρ' -> ρ = ρ'.
-Proof.
-  intros.
-  rewrite H in H0.
-  apply H0.
-Qed.
-
-Lemma Poss_eq_unique2: forall {T} ρs (ρ: Poss (VF T)) ρ', 
-  ρs = eq ρ -> ρs = eq ρ' -> ρ' = ρ.
-Proof.
-  intros.
-  rewrite H in H0.
-  assert(eq ρ ρ = eq ρ' ρ). { rewrite H0. reflexivity. }
-  rewrite <- H1.
-  reflexivity.
-Qed.
-
-Lemma SpinLock_Inv_in_R {T} : 
-  forall (i j : Name T), i <> j -> InvokeAny SpinLockImpl i ==> Rely j.
-Proof.
-  unfold InvokeAny, Guar, Rely, sub, subRelt; intros.
-  rename σ into σs.
-  rename ρ into ρs.
-  rename ρ0 into ρ.
-  destruct H0 as [Ret [m HInv]].
-  unfold TInvoke in HInv.
-  destruct HInv as [HIdle [HO [HU Hsig]]].
-  set ( σ :=
-     {| 
-        PState := ρ.(PState); 
-        PCalls := fun k =>
-          if (eqb i k) then CallPoss m
-          else ρ.(PCalls) k;
-        PRets := fun k =>
-          if (eqb i k) then RetIdle
-          else ρ.(PRets) k 
-      |}).
-  exists σ.
-  pose proof Poss_eq_inv i m ρs ρ σs σ H1 Hsig (ltac:(reflexivity)) as H0.
-  repeat split; simpl; try rewrite (eqb_nid _ _ H); auto.
-  inversion HO; exact (H3 j (ltac:(auto))).
-Qed.
-
-Lemma SpinLock_Ret_in_R {T} : 
-  forall (i j : Name T), i <> j -> ReturnAny SpinLockImpl i ==> Rely j.
-Proof.
-  unfold ReturnAny, Guar, Rely, sub, subRelt; intros.
-  rename σ into σs.
-  rename ρ into ρs.
-  rename ρ0 into ρ.
-  destruct H0 as [Ret [m HRet]].
-  unfold TReturn in HRet.
-  destruct HRet as [v [? [? [? ?]]]].
-  set ( σ :=
-     {| 
-        PState := ρ.(PState); 
-        PCalls := fun k =>
-          if (eqb i k) then CallDone m
-          else ρ.(PCalls) k;
-        PRets := fun k =>
-          if (eqb i k) then RetPoss m v
-          else ρ.(PRets) k 
-      |}).
-  exists σ.
-  unfold mapRetPoss in H4.
-  repeat split; simpl; try rewrite (eqb_nid _ _ H); auto.
-  + rewrite H4.
-    extensionality x.
-    apply propositional_extensionality.
-    admit.
-  + inversion H2.
-    exact (H6 j (ltac:(auto))).
-Admitted.
-
-(* Lemma SpinLock_init_in_P {T} : 
-  forall i (A: Type) m, Precs i A m (allIdle, (VE T).(Init)) (eq initPoss).
-Proof.
-  intros.
-  unfold Precs.
-  exists initPoss. split; auto.
-  destruct m; simpl; intros; try easy.
-  split. *)
-
-Lemma SpinLock_P_stable {T} : 
-  forall (i: Name T) A m, Stable (Rely i) (Precs i A m).
-Proof.
-  unfold Stable, stablePrec, PrecCompose, sub, subPrec.
-  intros.
-  destruct H as [s0 [ρ0 [? ?]]].
-  unfold Precs in *.
-  unfold Rely in H0.
-  destruct m.
-  + destruct H as [ρ0' [? ?]].
-    specialize (H0 _ H).
-    destruct H0 as [ρ' [? ?]].
-    exists ρ'. split; auto.
-    destruct_all.
-    assert((forall m : option(LockSig unit), PState ρ0' <> LockDef (Some i) m)). {
-      intros.
-      unfold LockOwned, LockRelRan, LockAcqRan in *.
-      destruct m; try easy.
-      dependent destruction l; easy.
-    }
-    specialize (H6 H10).
-    pose proof (H10 None).
-    pose proof (H10 (Some Rel)).
-    pose proof (H10 (Some Acq)).
-    unfold LockOwned, LockRelRan, LockAcqRan.
-    repeat split; easy.
-  + destruct H as [ρ0' [? ?]].
-    specialize (H0 _ H).
-    destruct H0 as [ρ' [? ?]].
-    exists ρ'. split; auto.
-    destruct_all.
-    specialize (H4 None).
-    specialize (H4 H1).
-    split; [exact H4 | ].
-    assert(snd s0 = snd s). {
-      specialize (H5 None).
-      apply H5, H1.
-    }
-    rewrite <- H9.
-    apply H8.
-Qed.
-
-(* Lemma SpinLock_Q_stable {T} : 
-  forall (i: Name T) A m, Stable (Rely i) (Posts i A m).
-Proof.
-  unfold Stable, stablePost, stableRelt, sub, subRelt, ReltCompose.
-  intros.
-  destruct H as [t0 [σ0 [? ?]]].
-  unfold Posts in *.
-  unfold Rely in H0.
-  intros.
-  specialize (H _ H1).
-  destruct H as [σ0' [? ?]].
-  specialize (H0 _ H).
-  destruct H0 as [σ' [? ?]].
-  exists σ'. split; [exact H0 | ].
-  destruct m.
-  + destruct_all.
-    specialize (H5 None).
-    pose proof (proj1 H5 H2).
-    easy.
-  + destruct_all.
-    specialize (H5 None).
-    pose proof (proj1 H5).
-    repeat split; try easy.
-    { apply (proj1 H7 H9). }
-    { rewrite <- H4. apply H10. }
-    { rewrite <- H3. apply H11. }
-    { rewrite <- H12, H8. reflexivity. }
-Qed. *)
-
-(* Lemma SpinLock_switch_code {T} : 
-  forall (i: Name T) A m1 B m2 v,
-    (prComp (Precs i A m1) (Posts i A m1 v)) <<- (Posts i A m1 v) <<- TReturn SpinLockImpl i m1 v ==> Precs i B m2.
-Proof.
-  intros.
-  unfold sub, subPrec, subRelt, ReltCompose, PrecCompose.
-  intros.
-  destruct H as [s1 [ρ1 [? ?]]].
-  destruct H as [s2 [ρ2 [? ?]]].
-Admitted. *)
-
-Lemma Rel_verify_aux' {T} :
-  forall (i: Name T) (s0: InterState F (VE T)) (ρs0: PossSet (VF T)) s1 ρs1,
-    (prComp (Precs i unit Rel) (TInvoke SpinLockImpl i unit Rel)) s0 ρs0 s1 ρs1 ->
-      exists ρ1, ρs1 = eq ρ1 /\
-        PState ρ1 = LockOwned i /\
-        PCalls ρ1 i = CallPoss Rel /\
-        PRets ρ1 i = RetIdle /\
-        snd s1 = CASDef (Some true) None /\
-        fst s1 i = Cont Rel (SpinLockImpl _ Rel).
-Proof.
-  intros.
-  unfold prComp, ReltCompose in H.
-  destruct H.
-  unfold Precs in H.
-  destruct H as [ρ [? [? ?]]].
-  unfold TInvoke in H0.
-  destruct H0 as [? [? [? ?]]].
-  exists {| 
-    PState := ρ.(PState); 
-    PCalls := fun j =>
-      if (eqb i j) then CallPoss Rel
-      else ρ.(PCalls) j;
-    PRets := fun j =>
-      if (eqb i j) then RetIdle
-      else ρ.(PRets) j
-  |}.
-  simpl.
-  rewrite (eqb_id i).
-  rewrite <- H2.
-  unfold TIdle in H0.
-  destruct H0.
-  split.
-  { pose proof Poss_eq_inv i Rel ρs0 ρ ρs1 
-    {| PState := PState ρ; 
-       PCalls := fun j : Name T => if i =? j then CallPoss Rel else PCalls ρ j; 
-       PRets := fun j : Name T => if i =? j then RetIdle else PRets ρ j |} H H5.
-    apply H7.
-    reflexivity. }
-  repeat split; try easy.
-  inversion H3; subst; simpl in *.
-  inversion H7; subst.
-  dependent destruction H5.
-  exact H12.
-Qed.
-
-Lemma Rel_verify_aux {T} :
-  forall (i: Name T) (s0: InterState F (VE T)) (ρs0: PossSet (VF T)) s1 ρs1,
-    (prComp (Precs i unit Rel) (TInvoke SpinLockImpl i unit Rel) ->> Rely i) s0 ρs0 s1 ρs1 ->
-      exists ρ1, ρs1 = eq ρ1 /\
-        PState ρ1 = LockOwned i /\
-        PCalls ρ1 i = CallPoss Rel /\
-        PRets ρ1 i = RetIdle /\
-        snd s1 = CASDef (Some true) None /\  
-        fst s1 i = Cont Rel (SpinLockImpl _ Rel).
-Proof.
-  intros.
-  unfold ReltCompose in H.
-  destruct H as [s2 [ρs2 [? ?]]].
-  pose proof Rel_verify_aux' i s0 ρs0 s2 ρs2 H.
-  destruct H1 as [ρ2 [? [? [? [? [? ?]]]]]].
-  unfold Rely in H0.
-  specialize (H0 _ H1).
-  destruct H0 as [ρ1 [? ?]].
-  destruct_all.
-  exists ρ1.
-  split; [exact H0 | ].
-  split; [apply (H9 None H2) |].
-  split.
-  { rewrite <- H7. apply H3. }
-  split.
-  { rewrite <- H8. apply H4. }
-  split. 
-  { pose proof (H10 None H2). rewrite <- H13. apply H5. }
-  rewrite <- H12. apply H6.
-Qed.
-
-Lemma Rel_verify_aux'' {T} :
-  forall (i: Name T) (s0: InterState F (VE T)) (ρs0: PossSet (VF T)) s1 ρs1,
-    (prComp (Precs i unit Rel) (TInvoke SpinLockImpl i unit Rel) ->> Rely i) s0 ρs0 s1 ρs1 ->
-      exists ρ0, ρs0 = eq ρ0 /\ PState ρ0 = LockOwned i /\ snd s0 = CASDef (Some true) None.
-Proof.
-  intros.
-  unfold prComp, ReltCompose in H.
-  destruct_all.
-  unfold Precs in H.
-  unfold PrecToRelt in H.
-  apply H.
-Qed.
-
-Lemma differ_pointwise_trans {A State} : forall (i: A) s1 s2 (s3: (A -> State)),
-  differ_pointwise s1 s2 i -> differ_pointwise s2 s3 i -> differ_pointwise s1 s3 i.
-Proof.
-  intros.
-  unfold differ_pointwise in *.
-  intros.
-  specialize (H j H1).
-  specialize (H0 j H1).
-  auto.
-  rewrite H0, H.
-  reflexivity.
-Qed.
-
-Lemma SpinLock_Rel_verified {T} : 
-  forall (i: Name T),
-    VerifyProg i (Rely i) (Guar i)
-      (prComp (Precs i unit Rel) (TInvoke SpinLockImpl i _ Rel) ->> Rely i)
-      (SpinLockImpl _ Rel)
-      (fun v => Posts i unit Rel v).
-Proof.
-  intros. simpl.
-  unfold SpinLockRel.
-  apply (lemBind (fun (_: bool) => 
-            (fun v : unit => Posts i unit Rel v) tt)).
-  + eapply weakenPost.
-    eapply (lemCall 
-      (Q := fun (s: InterState F (VE T)) (ρs: PossSet (VF T)) t σs =>
-        exists ρ σ, ρs = eq ρ /\ σs = eq σ /\
-        UnderThreadStep (fst s i) (Some (CallEv (CAS (Some true) None))) (fst t i) /\
-        Step (VE T) (snd s) (i, (CallEv (CAS (Some true) None))) (snd t) /\ 
-        PState σ = LockRelRan i /\
-        PCalls σ i = CallDone Rel /\
-        PRets σ i = RetIdle /\
-        True /\ True)   (* The following conditions are removed. Use True /\ True to avoid label changes  *)
-        (* (forall j, j <> i -> PCalls σ j = PCalls ρ j) /\
-        (forall j, j <> i -> PRets σ j = PRets ρ j)) *)
-      (S := fun v s ρs t σs =>
-        exists ρ σ, ρs = eq ρ /\ σs = eq σ /\ v = true /\
-        UnderThreadStep (fst s i) (Some (RetEv (CAS (Some true) None) true)) (fst t i) /\
-        (forall m, PState σ <> LockDef (Some i) m) /\
-        PCalls σ i = CallDone Rel /\
-        PRets σ i = RetPoss Rel tt /\
-        True /\ True)).   (* The following conditions are removed. Use True /\ True to avoid label changes  *)
-        (* (forall j, j <> i -> PCalls σ j = PCalls ρ j) /\
-        (forall j, j <> i -> PRets σ j = PRets ρ j))). *)
-    {
-      unfold Stable, stableRelt, sub, subRelt.
-      intros; simpl in *.
-      unfold ReltCompose in H.
-      rename ρ into ρs.
-      rename σ into σs.
-      destruct H as [s0 [ρs0 [? ?]]].
-      destruct H as [ρ [ρ0 [? [? ?]]]].
-      unfold Rely in H0.
-      specialize (H0 _ H1).
-      destruct H0 as [σ [? ?]].
-      exists ρ, σ.
-      split; [exact H |].
-      split; [exact H0 |].
-      destruct_all.
-      change (@fst (ThreadsSt T E F) (CASState T bool) t i) with 
-        (@fst (ThreadsSt T E LockSig) (@State T E (VE T)) t i).
-      rewrite <- H8.
-      split; [exact H2 |].
-      specialize (H6 _ H10).
-      change (@snd (ThreadsSt T E F) (CASState T bool) t) with 
-        (@snd (ThreadsSt T E LockSig) (@State T E (VE T)) t).
-      rewrite <- H6.
-      split; [ exact H9 |].
-      split; [ apply (H5 (Some Rel) H10) |].
-      split.
-      { unfold F in H11. rewrite H11 in H3. unfold F. rewrite H3. reflexivity. }
-      split.
-      { unfold F in H12. rewrite H12 in H4. unfold F. rewrite H4. reflexivity. }
-      easy.
-    }
-    { 
-      unfold Stable, stablePost, stableRelt, sub, subRelt.
-      intros; simpl in *.
-      unfold ReltCompose in H.
-      rename ρ into ρs.
-      rename σ into σs.
-      destruct H as [s0 [ρs0 [? ?]]].
-      destruct H as [ρ [ρ0 [? [? ?]]]].
-      unfold Rely in H0.
-      specialize (H0 _ H1).
-      destruct H0 as [σ [? ?]].
-      exists ρ, σ.
-      split; [exact H |].
-      split; [exact H0 |].
-      destruct_all.
-      split; [exact H2 |].
-      change (@fst (ThreadsSt T E F) (CASState T bool) t i) with 
-        (@fst (ThreadsSt T E LockSig) (@State T E (VE T)) t i).
-      rewrite <- H8.
-      split; [exact H9 |].
-      split; [apply H7, H10 |].
-      split.
-      { unfold F in H11. rewrite H11 in H3. unfold F. rewrite H3. reflexivity. }
-      split.
-      { unfold F in H12. rewrite H12 in H4. unfold F. rewrite H4. reflexivity. }
-      easy.
-    }
-    { 
-      unfold Commit.
-      intros.
-      unfold ReltToPrec in H.
-      destruct H as [s0 [ρs0 ?]].
-      pose proof Rel_verify_aux i s0 ρs0 s ρs H.
-      destruct H3 as [ρ [? ?]].
-      destruct_all.
-      remember
-      (fun σ: Poss (VF T) => 
-        PState σ = LockRelRan i /\
-        PCalls σ i = CallDone Rel /\
-        PRets σ i = RetIdle /\
-        differ_pointwise (PCalls ρ) (PCalls σ) i /\
-        differ_pointwise (PRets ρ) (PRets σ) i) as σs.
-      pose proof Poss_eq_inv3 _ _ _ _ _ _ Heqσs.
-      remember (
-        (MkPoss T LockSig (VF T)
-        (@LockRelRan (Name T) i)
-        (fun k : Name T =>
-      match @eqb (Name T) i k
-      return (PCall LockSig) with
-      | true => @CallDone LockSig unit Rel
-      | false => @PCalls T LockSig (VF T) ρ k
-      end)
-        (fun k : Name T =>
-      match @eqb (Name T) i k
-      return (PRet LockSig) with
-      | true => @RetIdle LockSig
-      | false => @PRets T LockSig (VF T) ρ k
-      end))) as σ.
-      exists σs.
-      split. { exists σ. rewrite H9. reflexivity. }
-      split. 
-      { intros. exists ρ. 
-        pose proof Poss_eq_unique _ _ _ H9 H10; subst σ0. 
-        split. { rewrite H3. reflexivity. }
-        apply (PossStepsStep i ρ σ σ).
-        { apply (PCommitCall i _ _ unit Rel); subst σ; simpl; try easy.
-          { rewrite H4. constructor. }
-          { rewrite eqb_id. reflexivity. }
-          { rewrite eqb_id. reflexivity. }
-        }
-        { intros. subst σ. simpl. rewrite (eqb_nid _ _ H11). reflexivity. }
-        { intros. subst σ. simpl. rewrite (eqb_nid _ _ H11). reflexivity. }
-        { constructor. }
-      }
-      split.
-      { exists ρ, σ.
-        repeat split; subst σ; simpl; try rewrite eqb_id; try easy.
-        (* { intros. rewrite (eqb_nid i j (ltac:(auto))). reflexivity. }
-        { intros. rewrite (eqb_nid i j (ltac:(auto))). reflexivity. } *)
-      }
-      unfold Guar.
-      intros.
-      pose proof Poss_eq_unique2 _ _ _ H3 H10; subst ρ0.
-      exists σ.
-      split; [exact H9 |].
-      unfold differ_pointwise in H0.
-      split. { intros. specialize (H0 _ H11); easy. }
-      split.
-      { intros. subst σ. simpl. rewrite (eqb_nid i j (ltac:(auto))). reflexivity. }
-      split.
-      { intros. subst σ. simpl. rewrite (eqb_nid i j (ltac:(auto))). reflexivity. }
-      split.
-      { intros. subst σ; simpl. rewrite H4 in H12. inversion H12; subst j; contradiction. }
-      split.
-      { intros. subst σ; simpl.
-        rewrite H4 in H12. inversion H12; subst j; contradiction. }
-      intros.
-      subst σ; intros; simpl.
-      { unfold LockRelRan. intro. inversion H13; subst; contradiction. }
-    }
-    {
-      unfold Commit; intros.
-      unfold ReltToPrec in H.
-      destruct H as [s0 [ρs0 ?]].
-      unfold ReltCompose in H at 1.
-      destruct H as [s1 [ρs1 ?]].
-      destruct H.
-      pose proof Rel_verify_aux i s0 ρs0 s1 ρs1 H.
-      clear H.
-      destruct H4 as [ρ1 [? ?]].
-      destruct_all.
-      assert(ρ1 = x). { apply (Poss_eq_unique2 _ _ _ H3 H). }
-      subst x.
-      rename x0 into ρ.
-      remember
-      (fun σ: Poss (VF T) => 
-        PState σ = LockUnowned /\
-        PCalls σ i = CallDone Rel /\
-        PRets σ i = RetPoss Rel tt /\
-        differ_pointwise (PCalls ρ) (PCalls σ) i /\
-        differ_pointwise (PRets ρ) (PRets σ) i) as σs.
-      pose proof Poss_eq_inv3 _ _ _ _ _ _ Heqσs.
-      remember
-      (MkPoss T LockSig (VF T) (@LockUnowned (Name T))
-      (fun k : Name T =>
-      match @eqb (Name T) i k return (PCall LockSig) with
-      | true => @CallDone LockSig unit Rel
-      | false => @PCalls T LockSig (VF T) ρ k
-      end)
-        (fun k : Name T =>
-      match @eqb (Name T) i k return (PRet LockSig) with
-      | true => @RetPoss LockSig unit Rel tt
-      | false => @PRets T LockSig (VF T) ρ k
-      end)) as σ.
-      exists σs.
-      split. { exists σ. rewrite H17; reflexivity. } 
-      split.
-      { intros. pose proof Poss_eq_unique _ _ _ H17 H18; subst σ0. 
-        exists ρ. split; [rewrite H9; reflexivity |].
-        apply (PossStepsStep i ρ σ σ).
-        { apply (PCommitRet i _ _ unit Rel tt); subst σ; simpl; try easy.
-          { unfold F in H12. rewrite H12. constructor. }
-          { rewrite eqb_id. reflexivity. }
-          { rewrite eqb_id. reflexivity. }
-        }
-        { intros. subst σ. simpl. rewrite (eqb_nid _ _ H19). reflexivity. }
-        { intros. subst σ. simpl. rewrite (eqb_nid _ _ H19). reflexivity. }
-        { constructor. }
-      }
-      split.
-      { exists ρ, σ.
-        assert(v = true).
-        { unfold F in H11.
-          rewrite H7 in H11.
-          inversion H11; subst.
-          change (@snd (ThreadsSt T E F) (@State T E (VE T)) s) with 
-            (@snd (ThreadsSt T E LockSig) (CASState T bool) s) in H2.
-          rewrite <- H23 in H2.
-          inversion H2; subst.
-          { dependent destruction H21; easy. }
-          { contradiction. }
-        }
-        subst v.
-        repeat split; subst σ; simpl; try rewrite eqb_id; try easy.
-        (* { intros. rewrite (eqb_nid i j (ltac:(auto))). reflexivity. }
-        { intros. rewrite (eqb_nid i j (ltac:(auto))). reflexivity. } *)
-      }
-      unfold Guar.
-      intros.
-      pose proof Poss_eq_unique2 _ _ _ H18 H9; subst ρ0.
-      exists σ.
-      split; [exact H17 |]. 
-      split.
-      { unfold differ_pointwise in H0. intros. specialize (H0 _ H19); easy. }
-      split.
-      { subst σ. simpl. intros. rewrite (eqb_nid i j (ltac:(auto))). reflexivity. }
-      split.
-      { subst σ. simpl. intros. rewrite (eqb_nid i j (ltac:(auto))). reflexivity. }
-      split.
-      { subst σ. simpl. unfold F in H12. rewrite H12.
-        intros; inversion H20; subst j; contradiction. }
-      split.
-      { subst σ. simpl. unfold F in H12. rewrite H12. intros. inversion H20; subst j; contradiction. }
-      intros.
-      subst σ; intros; simpl.
-      { unfold LockUnowned. intro. inversion H21; subst; contradiction. }
-    }
-    {
-      unfold sub, subRelt.
-      intros.
-      unfold ReltToPrec in H.
-      rename ρ into ρs.
-      rename σ into σs.
-      destruct H as [s0 [ρs0 ?]].
-      unfold ReltCompose in H at 2.
-      destruct H.
-      pose proof Rel_verify_aux i s ρs s0 ρs0 H.
-      destruct H1 as [ρ0 [? ?]].
-      destruct H0 as [s1 [ρs1 ?]].
-      destruct H0.
-      destruct H0 as [ρ0_ [ρ1 [? [? ?]]]].
-      pose proof Poss_eq_unique2 _ _ _ H0 H1; subst ρ0_.
-      destruct H3 as [ρ1_ [σ [? [? ?]]]].
-      pose proof Poss_eq_unique2 _ _ _ H3 H4; subst ρ1_.
-      unfold Posts. intros.
-      pose proof Rel_verify_aux'' i s ρs s0 ρs0 H.
-      destruct H8 as [ρ [? ?]].
-      exists ρ, σ.
-      split; [exact H8 |].
-      split; [exact H6 |].
-      split; [exact (proj1 H9) |].
-      destruct_all.
-      split; [exact H16 |].
-      split; [exact H18|].
-      split; [exact H17 |].
-      unfold F in H5. rewrite H14 in H5.
-      inversion H5; subst.
-      dependent destruction H30.
-      unfold F in H15. rewrite H32 in H15.
-      inversion H15; subst.
-      dependent destruction H8.
-      unfold call, ret in x.
-      dependent destruction x.
-      rewrite ProgramFacts.frobProgId in x at 1. unfold ProgramFacts.frobProgram in x. simpl in x.
-      inversion x.
-      dependent destruction H1.
-      rewrite H29.
-      rewrite (ProgramFacts.frobProgId (@Return (CASSig bool) bool true;; Return tt)).
-      unfold ProgramFacts.frobProgram.
-      simpl. reflexivity.
-    }
-  + intros.
-    apply lemRet.
-    intros.
-    destruct v0.
-    easy.
-Qed.
-
-Lemma SpinLock_Acq_verified {T} : 
-  forall (i: Name T),
-    VerifyProg i (Rely i) (Guar i)
-      (prComp (Precs i unit Acq) (TInvoke SpinLockImpl i _ Acq) ->> Rely i)
-      (SpinLockImpl _ Acq)
-      (fun v => Posts i unit Acq v).
-Proof.
-  intros.
-  simpl.
-  unfold SpinLockAcq.
-Admitted.
-
-Lemma SpinLock_all_verified {T} : 
-  forall (i: Name T) A m,
-    VerifyProg i (Rely i) (Guar i)
-      (prComp (Precs i A m) (TInvoke SpinLockImpl i _ m) ->> Rely i)
-      (SpinLockImpl _ m)
-      (fun v => Posts i A m v).
-Proof.
-  intros.
-  destruct m eqn : I.
-  + apply SpinLock_Acq_verified.
-  + apply SpinLock_Rel_verified.
-Qed.
-
-End SpinLockNormal.
-
-
-
-
-Module SpinLockUB.
-
-Definition E := CASSig bool.
-Definition F := LockSig.
-Definition acf T := @LockActiveMap T.
-Definition HAcf T : @acf_sound T F lockSpec (acf T) := @LockActiveMapSound T.
-Definition VE T : Spec T E:= @casSpec T bool.
-Definition VF T := @lockSpec T.
-Definition VFU T := SpecWithUB (@lockSpec T) (acf T) (HAcf T).
-Definition ReltU T := Relt (VE T) (VFU T).
-Definition Relt T := Relt (VE T) (VF T).
-Definition PrecU T := Prec (VE T) (VFU T).
-Definition Prec T := Prec (VE T) (VF T).
-Definition PostU T := Post (VE T) (VFU T).
-Definition Post T := Post (VE T) (VF T).
-Definition UState T := State (VFU T).
-
-Definition Precs {T} i A (m : LockSig A) : @PrecU T :=
-  fun s ρs => exists ρ, ρs = eq ρ /\
-    match m with
-    | Acq =>
-        PState ρ = inl (LockOwned i) \/ 
-        PState ρ = inl (LockRelRan i) \/ 
-        PState ρ = inl (LockAcqRan i) \/
-        exists a, PState ρ = inr (UBState_, a)
-    | Rel =>
-        PState ρ <> inl (LockOwned i) /\
-        (StateWithUB_acf _ (acf T) (PState ρ) i = None)
-    end.
-
-Definition Posts {T} i A (m : LockSig A) : @PostU T A :=
-  fun _ s ρs t σs => exists ρ σ, ρs = eq ρ /\ σs = eq σ /\
-    match m with
-    | Acq =>
-        exists a, PState σ = inr (UBState_, a) /\
-        PCalls σ i = CallDone Acq /\
-        PRets σ i = RetPoss Acq tt
-    | Rel =>
-        exists a, PState σ = inr (UBState_, a) /\
-        PCalls σ i = CallDone Rel /\
-        PRets σ i = RetPoss Rel tt
-    end.
-
-(* Definition Rely {T} i := ReltWithUB (VF := (VF T)) (acf T) (HAcf T) (SpinLockNormal.Rely i).
-Definition Guar {T} i := ReltWithUB (VF := (VF T)) (acf T) (HAcf T) (SpinLockNormal.Guar i).
-Ltac unfold_rely H := unfold Rely, ReltWithUB, SpinLockNormal.Rely in H.
-Ltac unfold_guar H := unfold Guar, ReltWithUB, SpinLockNormal.Guar in H. *)
-
-Definition Rely {T} i : ReltU T :=
-  fun s ρs t σs => forall ρ, ρs = eq ρ -> exists σ, σs = eq σ /\
-    (PCalls ρ i = PCalls σ i) /\
-    (PRets ρ i = PRets σ i) /\
-    (forall m, PState ρ = inl (LockDef (Some i) m) -> 
-      (PState σ = inl (LockDef (Some i) m) \/ 
-      (exists a, PState σ = inr (UBState_, a)))) /\
-    True /\
-    (* (forall m, PState ρ = inl (LockDef (Some i) m) -> snd s = snd t) /\ *)
-    ((forall m, PState ρ <> inl (LockDef (Some i) m)) -> (forall m, PState σ <> inl (LockDef (Some i) m))) /\
-    ((exists a, PState ρ = inr (UBState_, a)) -> (exists a', PState σ = inr (UBState_, a'))) /\
-    (fst s i = fst t i) /\
-    (StateWithUB_acf _ (acf T) (PState ρ) i = StateWithUB_acf _ (acf T) (PState σ) i).
-
-Definition Guar {T} i : ReltU T :=
-  fun s ρs t σs => forall ρ, ρs = eq ρ -> exists σ, σs = eq σ /\
-    (forall j, j <> i -> fst s j = fst t j) /\
-    (forall j, j <> i -> PCalls ρ j = PCalls σ j) /\
-    (forall j, j <> i -> PRets ρ j = PRets σ j) /\
-    (forall j, j <> i ->
-      forall m, PState ρ = inl (LockDef (Some j) m) ->
-        (PState σ = inl (LockDef (Some j) m) \/ 
-        (exists a, PState σ = inr (UBState_, a)))) /\
-    True /\
-    (* (forall j, j <> i -> 
-      forall m, PState ρ = inl (LockDef (Some j) m) -> snd s = snd t) /\ *)
-    (forall j, j <> i -> 
-      ((forall m, PState ρ <> inl (LockDef (Some j) m)) -> (forall m, PState σ <> inl (LockDef (Some j) m)))) /\
-    ((exists a, PState ρ = inr (UBState_, a)) -> (exists a', PState σ = inr (UBState_, a'))) /\
-    (forall j, j <> i -> (StateWithUB_acf _ (acf T) (PState ρ) j = StateWithUB_acf _ (acf T) (PState σ) j)).
-
-Lemma Poss_eq_unique: forall {T} ρs (ρ: Poss (VFU T)) ρ', 
-  ρs = eq ρ -> ρs ρ' -> ρ = ρ'.
-Proof.
-  intros.
-  rewrite H in H0.
-  apply H0.
-Qed.
-
-Lemma Poss_eq_unique2: forall {T} ρs (ρ: Poss (VFU T)) ρ', 
-  ρs = eq ρ -> ρs = eq ρ' -> ρ' = ρ.
-Proof.
-  intros.
-  rewrite H in H0.
-  assert(eq ρ ρ = eq ρ' ρ). { rewrite H0. reflexivity. }
-  rewrite <- H1.
-  reflexivity.
-Qed.
-
-Lemma SpinLock_G_in_R {T} : 
-  forall (i j : Name T), i <> j -> Guar i ==> Rely j.
-Proof.
-  unfold Guar, Rely, sub, subRelt.
-  intros.
-  specialize (H0 _ H1).
-  destruct_all.
-  rename ρ into ρs.
-  rename σ into σs.
-  rename x into σ.
-  rename ρ0 into ρ.
-  exists σ.
-  assert(j <> i) by auto.
-  specialize (H2 _ H10).
-  specialize (H3 _ H10).
-  specialize (H4 _ H10).
-  specialize (H5 _ H10).
-  specialize (H7 _ H10).
-  specialize (H9 _ H10).
-  repeat split; intros; simpl; try easy.
-  + specialize (H5 _ H11).
-    destruct H5.
-    - left. easy.
-    - right. destruct_all. exists x. apply H5.
-  + specialize (H7 H11).
-    apply H7.
-  + apply (H8 H11).
-Qed.
-
-Lemma Rel_verify_aux1 {T} :
-  forall (i: Name T) (s0: InterState F (VE T)) (ρs0: PossSet (VFU T)) s1 ρs1,
-    (prComp (Precs i unit Rel) (TInvoke SpinLockImpl i unit Rel)) s0 ρs0 s1 ρs1 ->
-      exists ρ1, ρs1 = eq ρ1 /\
-        PState ρ1 <> inl (LockOwned i) /\
-        (StateWithUB_acf _ (acf T) (PState ρ1) i = None) /\
-        PCalls ρ1 i = CallPoss Rel /\
-        PRets ρ1 i = RetIdle /\
-        fst s1 i = Cont Rel (SpinLockImpl _ Rel).
-Proof.
-  intros.
-  unfold prComp, ReltCompose in H.
-  destruct H.
-  unfold Precs in H.
-  destruct H as [ρ0 [? ?]].
-  unfold TInvoke in H0.
-  destruct H0 as [? [? [? ?]]].
-  exists {| 
-    PState := ρ0.(PState); 
-    PCalls := fun j =>
-      if (eqb i j) then CallPoss Rel
-      else ρ0.(PCalls) j;
-    PRets := fun j =>
-      if (eqb i j) then RetIdle
-      else ρ0.(PRets) j
-  |}.
-  simpl.
-  rewrite (eqb_id i).
-  unfold TIdle in H0.
-  destruct H0.
-  split.
-  { pose proof SpinLockNormal.Poss_eq_inv i Rel ρs0 ρ0 ρs1
-    {| PState := PState ρ0; 
-       PCalls := fun j : Name T => if i =? j then CallPoss Rel else PCalls ρ0 j; 
-       PRets := fun j : Name T => if i =? j then RetIdle else PRets ρ0 j |} H H4.
-    apply H6.
-    reflexivity. }
-  repeat split; try easy.
-  inversion H2; subst; simpl in *.
-  inversion H6; subst.
-  dependent destruction H4.
-  exact H11.
-Qed.
-
-Lemma LockUnowned_Rely {T} :
-  forall (i: Name T) (s0: InterState F (VE T)) (ρs0: PossSet (VFU T)) s1 ρs1 ρ0,
-    ρs0 = eq ρ0 ->
-    Rely i s0 ρs0 s1 ρs1 ->
-    PState ρ0 <> inl (LockOwned i) ->
-    (exists ρ1, (ρs1 = eq ρ1) /\ PState ρ1 <> inl (LockOwned i)).
-Proof.
-  intros.
-  unfold Rely in H0.
-  specialize (H0 _ H).
-  destruct_all.
-  rename x into ρ1.
-  exists ρ1.
-  split; [exact H0 |].
-  destruct (PState ρ0).
-  + destruct s as [j m].
-    destruct j.
-    - rename n into j.
-      destruct (classicT (i = j)).
-      * subst j.
-        specialize (H4 m (ltac:(auto))).
-        destruct m.
-        { destruct H4.
-          rewrite H4. easy. 
-          destruct_all.
-          rewrite H4. easy.
-        }
-        contradiction.
-      * apply H6. intros. intro.
-        inversion H10. rewrite H12 in n. contradiction.
-    - apply H6. easy.
-  + assert(forall m : option (LockSig unit), inr p <> inl (LockDef (Some i) m)) by (intros; easy).
-    apply (H6 H10).
-Qed.
-
-Lemma Rel_verify_aux2 {T} :
-  forall (i: Name T) (s0: InterState F (VE T)) (ρs0: PossSet (VFU T)) s1 ρs1,
-    (prComp (Precs i unit Rel) (TInvoke SpinLockImpl i unit Rel) ->> Rely i) s0 ρs0 s1 ρs1 ->
-      exists ρ1, ρs1 = eq ρ1 /\
-        PState ρ1 <> inl (LockOwned i) /\
-        (StateWithUB_acf _ (acf T) (PState ρ1) i = None) /\
-        PCalls ρ1 i = CallPoss Rel /\
-        PRets ρ1 i = RetIdle /\
-        fst s1 i = Cont Rel (SpinLockImpl _ Rel).
-Proof.
-  intros.
-  unfold ReltCompose in H.
-  destruct H as [s2 [ρs2 [? ?]]].
-  pose proof Rel_verify_aux1 i s0 ρs0 s2 ρs2 H.
-  destruct H1 as [ρ2 [? [? [? [? ?]]]]].
-  pose proof LockUnowned_Rely _ _ _ _ _ _ H1 H0 H2.
-  unfold Rely in H0.
-  specialize (H0 _ H1).
-  destruct H0 as [ρ1 [? ?]].
-  destruct_all.
-  pose proof Poss_eq_unique2 _ _ _ H6 H0; subst x.
-  exists ρ1.
-  split; [exact H0 | ].
-  split; [exact H16 |].
-  split.
-  { rewrite <- H15. apply H3. }
-  split.
-  { rewrite <- H7. apply H4. }
-  split.
-  { rewrite <- H9. apply H5. }
-  rewrite <- H14. apply H8.
-Qed.
-
-Lemma Rel_verify_aux3 {T} :
-  forall (i: Name T) (s0: InterState F (VE T)) (ρs0: PossSet (VFU T)) s1 ρs1,
-    ((prComp (Precs i unit Rel) (TInvoke SpinLockImpl i unit Rel) ->> Rely i) ->>
-    (fun s ρs t σs =>
-        exists ρ σ, ρs = eq ρ /\ σs = eq σ /\
-        UnderThreadStep (fst s i) (Some (CallEv (CAS (Some true) None))) (fst t i) /\
-        (exists a, PState σ = inr (UBState_, a) /\ (a i = Some (existT (fun A => LockSig A) unit Rel))) /\
-        PCalls σ i = CallDone Rel /\
-        PRets σ i = RetIdle)) s0 ρs0 s1 ρs1 -> 
-    exists ρ1, ρs1 = eq ρ1 /\
-      (exists a, PState ρ1 = inr (UBState_, a) /\ (a i = Some (existT (fun A => LockSig A) unit Rel))) /\
-      PCalls ρ1 i = CallDone Rel /\
-      PRets ρ1 i = RetIdle /\
-      fst s1 i = UCall Rel (CAS (Some true) None) (fun x1 : bool => Return x1;; Return tt).
-Proof.
-  intros.
-  unfold ReltCompose in H at 1.
-  destruct H as [s2 [ρs2 [? ?]]].
-  pose proof Rel_verify_aux2 i s0 ρs0 s2 ρs2 H.
-  destruct H1 as [ρ2 [? [? [? [? ?]]]]].
-  destruct H0 as [ρ2' [ρ1 [? [? ?]]]].
-  pose proof Poss_eq_unique2 _ _ _ H0 H1; subst ρ2'.
-  exists ρ1.
-  split; [exact H6 |].
-  destruct_all.
-  split. { exists x. easy. }
-  split; [exact H10 |].
-  split; [exact H11 |].
-  rewrite H8 in H7.
-  inversion H7; subst.
-  dependent destruction H14.
-  unfold call, ret in x.
-  rewrite ProgramFacts.frobProgId in x at 1. unfold ProgramFacts.frobProgram in x. simpl in x.
-  inversion x.
-  dependent destruction H6.
-  rewrite H18.
-  reflexivity.
-Qed.
-
-Lemma Rel_verify_aux4 {T} :
-  forall (i: Name T) (s0: InterState F (VE T)) (ρs0: PossSet (VFU T)) s1 ρs1 v,
-    (((prComp (Precs i unit Rel) (TInvoke SpinLockImpl i unit Rel) ->> Rely i) ->>
-    (fun (s: InterState F (VE T)) (ρs: PossSet (VFU T)) t σs =>
-        exists ρ σ, ρs = eq ρ /\ σs = eq σ /\
-        UnderThreadStep (fst s i) (Some (CallEv (CAS (Some true) None))) (fst t i) /\
-        (exists a, PState σ = inr (UBState_, a) /\ (a i = Some (existT (fun A => LockSig A) unit Rel))) /\
-        PCalls σ i = CallDone Rel /\
-        PRets σ i = RetIdle)) ->>
-    (fun s ρs t (σs: PossSet (VFU T)) =>
-        exists ρ σ, ρs = eq ρ /\ σs = eq σ /\
-        UnderThreadStep (fst s i) (Some (RetEv (CAS (Some true) None) v)) (fst t i) /\
-        (exists a, PState σ = inr (UBState_, a) /\ a i = None) /\
-        PCalls σ i = CallDone Rel /\
-        PRets σ i = RetPoss Rel tt)) s0 ρs0 s1 ρs1 -> 
-    exists ρ1, ρs1 = eq ρ1 /\
-        fst s1 i = Cont Rel (Return tt) /\
-        (exists a, PState ρ1 = inr (UBState_, a) /\ a i = None) /\
-        PCalls ρ1 i = CallDone Rel /\
-        PRets ρ1 i = RetPoss Rel tt.
-Proof.
-  intros.
-  unfold ReltCompose in H at 1.
-  destruct H as [t [σs [? ?]]].
-  pose proof Rel_verify_aux3 i s0 ρs0 t σs H.
-  clear H.
-  destruct H1 as [σ [? ?]].
-  destruct_all.
-  rename x into a.
-  rename x0 into σ'.
-  rename x1 into ρ1.
-  pose proof Poss_eq_unique2 _ _ _ H0 H; subst σ'.
-  exists ρ1.
-  destruct_all.
-  split; [exact H6 |].
-  split.
-  { rewrite H4 in H7. inversion H7; subst.
-    dependent destruction H13.
-    dependent destruction H16.
-    rewrite H18.
-    rewrite (ProgramFacts.frobProgId (Return v;; Return tt)).
-    simpl. reflexivity.
-  }
-  split. { exists x2. easy. }
-  split; [exact H9 |].
-  exact H10.
-Qed.
-
-Lemma SpinLock_Rel_verified {T} : 
-  forall (i: Name T),
-    VerifyProg i (Rely i) (Guar i)
-      (prComp (Precs i unit Rel) (TInvoke SpinLockImpl i _ Rel) ->> Rely i)
-      (SpinLockImpl _ Rel)
-      (fun v => Posts i unit Rel v).
-Proof.
-  intros; simpl.
-  apply (lemBind (fun (_: bool) => 
-            (fun v : unit => Posts i unit Rel v) tt)).
-  + eapply weakenPost.
-    eapply (lemCall 
-      (Q := fun (s: InterState F (VE T)) (ρs: PossSet (VFU T)) t σs =>
-        exists ρ σ, ρs = eq ρ /\ σs = eq σ /\
-        UnderThreadStep (fst s i) (Some (CallEv (CAS (Some true) None))) (fst t i) /\
-        (* Step (VE T) (snd s) (i, (CallEv (CAS (Some true) None))) (snd t) /\  *)
-        (exists a, PState σ = inr (UBState_, a) /\ (a i = Some (existT (fun A => LockSig A) unit Rel))) /\
-        PCalls σ i = CallDone Rel /\
-        PRets σ i = RetIdle)
-      (S := fun v s ρs t σs =>
-        exists ρ σ, ρs = eq ρ /\ σs = eq σ /\
-        UnderThreadStep (fst s i) (Some (RetEv (CAS (Some true) None) v)) (fst t i) /\
-        (exists a, PState σ = inr (UBState_, a) /\ a i = None) /\
-        PCalls σ i = CallDone Rel /\
-        PRets σ i = RetPoss Rel tt)).
-    { unfold Stable, stableRelt, sub, subRelt, ReltCompose.
-      intros.
-      rename ρ into ρs.
-      rename σ into σs.
-      destruct H as [s1 [ρs1 ?]].
-      destruct H.
-      destruct H as [ρ [ρ1 [? [? ?]]]].
-      unfold Rely in H0.
-      specialize (H0 _ H1).
-      destruct H0 as [σ [? ?]].
-      exists ρ, σ.
-      split; [exact H |].
-      split; [exact H0 |].
-      destruct_all.
-      unfold F. rewrite <- H9.
-      split; [easy |].
-      split.
-      { assert((exists a : ActiveMap T LockSig, PState ρ1 = inr (UBState_, a))).
-        { exists x. easy. }
-        specialize (H8 H15).
-        destruct H8 as [a' ?].
-        exists a'.
-        split; [ easy |].
-        unfold F in H11. rewrite H11 in H10.
-        rewrite H8 in H10.
-        unfold StateWithUB_acf in H10.
-        rewrite <- H10.
-        apply H14.
-      }
-      rewrite <- H3, <- H4.
-      easy.
-    }
-    {
-      unfold Stable, stablePost, stableRelt, sub, subRelt, ReltCompose.
-      intros.
-      rename ρ into ρs.
-      rename σ into σs.
-      destruct H as [s1 [ρs1 ?]].
-      destruct H.
-      destruct H as [ρ [ρ1 [? [? ?]]]].
-      unfold Rely in H0.
-      specialize (H0 _ H1).
-      destruct H0 as [σ [? ?]].
-      exists ρ, σ.
-      split; [exact H |].
-      split; [exact H0 |].
-      destruct_all.
-      unfold F. rewrite <- H9.
-      split; [easy |].
-      split.
-      { assert((exists a : ActiveMap T LockSig, PState ρ1 = inr (UBState_, a))).
-        { exists x. easy. }
-        specialize (H8 H15).
-        destruct H8 as [a' ?].
-        exists a'.
-        split; [ easy |].
-        unfold F in H11. rewrite H11 in H10.
-        rewrite H8 in H10.
-        unfold StateWithUB_acf in H10.
-        rewrite <- H10.
-        apply H14.
-      }
-      rewrite <- H3, <- H4.
-      easy.
-    }
-    {
-      unfold Commit.
-      intros.
-      unfold ReltToPrec in H.
-      destruct H as [s0 [ρs0 ?]].
-      pose proof Rel_verify_aux2 i s0 ρs0 s ρs H.
-      destruct H3 as [ρ [? [? [? [? ?]]]]].
-      remember (
-        MkPoss T F (VFU T)
-        (inr (UBState_, fun j => if i =? j then Some (existT (fun A => LockSig A) unit Rel) else (StateWithUB_acf _ (acf T) (PState ρ) j)))
-        (fun j => if i =? j then CallDone Rel else PCalls ρ j)
-        (fun j => if i =? j then RetIdle else PRets ρ j)) as σ.
-      exists (eq σ).
-      split. { exists σ. reflexivity. }
-      split.
-      { intros. exists ρ.
-        split. { rewrite H3. reflexivity. }
-        subst σ0.
-        apply (PossStepsStep i ρ σ σ).
-        { apply (PCommitCall i _ _ unit Rel); subst σ; simpl; try easy.
-          { destruct (PState ρ).
-            { constructor.
-              { intros. intro. inversion H8; subst. contradiction. }
-              { constructor. 
-                { unfold StateWithUB_acf in H5. apply H5. }
-                { rewrite eqb_id. reflexivity. }
-                { apply differ_pointwise_trivial. }
-              }
-            }
-            { destruct p. destruct u. constructor. constructor.
-              { unfold StateWithUB_acf in H5. apply H5. }
-              { rewrite eqb_id. reflexivity. }
-              { apply differ_pointwise_trivial. }
-            }
-          }
-          { rewrite eqb_id. reflexivity. }
-          { rewrite eqb_id. reflexivity. }
-        }
-        { intros. subst σ. simpl. rewrite (eqb_nid _ _ H8). reflexivity. }
-        { intros. subst σ. simpl. rewrite (eqb_nid _ _ H8). reflexivity. }
-        { constructor. }
-      }
-      split.
-      { exists ρ, σ.
-        repeat split; subst σ; simpl; try rewrite eqb_id; try easy.
-        eexists.
-        split. { reflexivity. }
-        simpl. rewrite eqb_id. reflexivity.
-      }
-      { unfold Guar.
-        intros.
-        pose proof Poss_eq_unique2 _ _ _ H8 H3; subst ρ0.
-        exists σ.
-        split; [reflexivity |].
-        split. 
-        { intros. unfold differ_pointwise in H0. specialize (H0 _ H9). easy. }
-        split.
-        { subst σ. simpl. intros. rewrite (eqb_nid i j (ltac:(auto))). reflexivity. }
-        split.
-        { subst σ. simpl. intros. rewrite (eqb_nid i j (ltac:(auto))). reflexivity. }
-        split.
-        { intros. subst σ. simpl.
-          right. 
-          eexists. reflexivity.
-        }
-        split; [ easy |].
-        split. { intros. subst σ. easy. }
-        split.
-        { intros. subst σ. simpl. eexists. reflexivity. }
-        { intros. subst σ. simpl. rewrite (eqb_nid i j (ltac:(auto))). reflexivity. }
-      }
-    }
-    {
-      unfold Commit.
-      intros.
-      unfold ReltToPrec in H.
-      destruct H as [s0 [ρs0 ?]].
-      pose proof Rel_verify_aux3 i s0 ρs0 s ρs H.
-      clear H.
-      destruct H3 as [ρ [? [? [? [? ?]]]]].
-      destruct H3 as [a [? ?]].
-      remember (
-        MkPoss T F (VFU T)
-        (inr (UBState_, fun j => if i =? j then None else (StateWithUB_acf _ (acf T) (PState ρ) j)))
-        (fun j => if i =? j then CallDone Rel else PCalls ρ j)
-        (fun j => if i =? j then RetPoss Rel tt else PRets ρ j)) as σ.
-      exists (eq σ).
-      split. { exists σ. reflexivity. }
-      split.
-      { intros. exists ρ.
-        split. { rewrite H. reflexivity. }
-        subst σ0.
-        apply (PossStepsStep i ρ σ σ).
-        { apply (PCommitRet i _ _ unit Rel tt); subst σ; simpl; try easy.
-          { rewrite H3. constructor. constructor.
-            { apply H7. }
-            { rewrite eqb_id. reflexivity. }
-            { apply differ_pointwise_trivial. }
-        }
-        { rewrite eqb_id. reflexivity. }
-        { rewrite eqb_id. reflexivity. }
-        }
-        { intros. subst σ. simpl. rewrite (eqb_nid _ _ H8). reflexivity. }
-        { intros. subst σ. simpl. rewrite (eqb_nid _ _ H8). reflexivity. }
-        { constructor. }
-      }
-      split.
-      { exists ρ, σ.
-        unfold F in H1. rewrite H6 in H1. inversion H1; subst.
-        dependent destruction H9.
-        dependent destruction H12.
-        unfold F. rewrite H6.
-        repeat split; simpl; try rewrite eqb_id; try easy.
-        eexists. split; [reflexivity |].
-        simpl. rewrite eqb_id. reflexivity.
-      }
-      { unfold Guar.
-        intros.
-        pose proof Poss_eq_unique2 _ _ _ H8 H; subst ρ0.
-        exists σ.
-        split; [reflexivity |].
-        split. 
-        { intros. unfold differ_pointwise in H0. specialize (H0 _ H9). easy. }
-        split.
-        { subst σ. simpl. intros. rewrite (eqb_nid i j (ltac:(auto))). reflexivity. }
-        split.
-        { subst σ. simpl. intros. rewrite (eqb_nid i j (ltac:(auto))). reflexivity. }
-        split.
-        { intros. subst σ. simpl.
-          right. 
-          eexists. reflexivity.
-        }
-        split; [ easy |].
-        split. { intros. subst σ. easy. }
-        split.
-        { intros. subst σ. simpl. eexists. reflexivity. }
-        { intros. subst σ. simpl. rewrite (eqb_nid i j (ltac:(auto))). reflexivity. }
-      }
-    }
-    {
-      unfold sub, subRelt.
-      intros.
-      rename ρ into ρs.
-      rename σ into σs.
-      rewrite <- LogicFacts.reltCompAssoc in H.
-      pose proof Rel_verify_aux4 i s ρs t σs v H.
-      assert(exists ρ, ρs = eq ρ).
-      { unfold ReltCompose in H. destruct_all. unfold prComp in H.
-        destruct H.
-        unfold Precs in H.
-        destruct H as [ρ0 [? ?]].
-        exists ρ0. rewrite H. reflexivity. 
-      }
-      clear H.
-      destruct H0 as [σ [? ?]].
-      unfold Posts.
-      destruct H1 as [ρ ?].
-      destruct_all.
-      exists ρ, σ.
-      repeat split; try easy.
-      exists x. easy.
-    }
-  + intros.
-    constructor.
-    easy. 
-Qed.
-
-End SpinLockUB.
-
-Module SpinLockAll.
-
